Updated definitions for directed congruence

formalization/DirectedCong.v
@@ -39,79 +39,6 @@ Reserved Notation "P '⇛' Q" (no associativity, at level 1).
 Reserved Notation "M '!⇛' N" (no associativity, at level 1).
 Reserved Notation "s '$⇛' r" (no associativity, at level 1).
 
-(* Inductive directed_congruence : process -> process -> Prop :=
-  (* links *)
-  | dc_cong_link : forall ml1 ml2 mr1 mr2,
-      ml1 !⇛ ml2 -> mr1 !⇛ mr2 -> (link ml1 mr1) ⇛ (link ml2 mr2)
-  | dc_link : forall ml1 ml2 mr1 mr2,
-      ml1 !⇛ ml2 -> mr1 !⇛ mr2 -> (link ml1 mr1) ⇛ (link mr2 ml2)
-
-  (* cuts *)
-  | dc_cut_comm : forall P P' Q Q', 
-      P ⇛ P' -> Q ⇛ Q' -> (cut P Q) ⇛ (cut Q' P')
-  | dc_cut_assoc_l : forall P (* P' *) P'' Q Q' R R' L L',
-      L ⇛ (cut P Q) (* (cut P Q) *) (* -> ~ (1 ∈ P) -> P' ⇛ P *) (* P ⇛ P' *) ->
-      P'' = down (rename_process P swap01) (* down (rename_process P' swap01) *) ->
-      Q' = rename_process Q swap01 ->
-      R' = rename_process (up R) swap01 ->
-      (cut Q' R') ⇛ L' ->
-      (cut L R) ⇛ (cut P'' L')
-  | dc_cut_assoc_l_comm : forall P P' P'' Q Q' R R' L L',
-      L ⇛ (cut P Q) -> ~ (1 ∈ P) -> P ⇛ P' ->
-      P'' = down (rename_process P' swap01) ->
-      Q' = rename_process Q swap01 ->
-      R' = rename_process (up R) swap01 ->
-      (cut Q' R') ⇛ L' ->
-      (cut L R) ⇛ (cut L' P'')
-  (* these rules are necessary to ensure admissibility of symmetry *)
-  | dc_cut_assoc_r : forall P P' Q Q' R R' R'' L L',
-      L ⇛ (cut Q R) -> ~ (1 ∈ R) -> R ⇛ R' ->
-      P' = rename_process (up P) swap01 ->
-      Q' = rename_process Q swap01 ->
-      R'' = down (rename_process R' swap01) ->
-      (cut P' Q') ⇛ L' ->
-      (cut P L) ⇛ (cut L' R'')
-  | dc_cut_assoc_r_comm : forall P P' Q Q' R R' R'' L L',
-      L ⇛ (cut Q R) -> ~ (1 ∈ R) -> R ⇛ R' ->
-      P' = rename_process (up P) swap01 ->
-      Q' = rename_process Q swap01 ->
-      R'' = down (rename_process R' swap01) ->
-      (cut P' Q') ⇛ L' ->
-      (cut P L) ⇛ (cut R'' L')
-  | dc_cong_cut : forall P P' Q Q', P ⇛ P' -> Q ⇛ Q' -> (cut P Q) ⇛ (cut P' Q')
-
-  (* seqs *)
-  | dc_cong_seq : forall P P' s s', P ⇛ P' -> s $⇛ s' -> (seq P s) ⇛ (seq P' s')
-
-  (* stop *)
-  | dc_stop : stop ⇛ stop
-where
-  "P '⇛' Q" := (directed_congruence P Q)
-
-with directed_congruence_message : message -> message -> Prop :=
-  | dc_cong_prefix : forall s s', s $⇛ s' -> (prefix s) !⇛ (prefix s')
-  | dc_cong_reflM : forall m, m !⇛ m
-where
-  "M '!⇛' N" := (directed_congruence_message M N)
-
-with directed_congruence_statement : statement -> statement -> Prop :=
-  | dc_cong_choose_l : forall P P',
-                        P ⇛ P' ->
-                        (choose_left P) $⇛ (choose_left P')
-  | dc_cong_choose_r : forall P P',
-                        P ⇛ P' ->
-                        (choose_right P) $⇛ (choose_right P')
-  | dc_cong_choice : forall P P' Q Q',
-                      P ⇛ P' -> Q ⇛ Q' -> (offer_choice P Q) $⇛ (offer_choice P' Q')
-  | dc_cong_send : forall P P' Q Q',
-                    P ⇛ P' -> Q ⇛ Q' -> (send P Q) $⇛ (send P' Q')
-  | dc_cong_receive : forall P P', P ⇛ P' -> (receive P) $⇛ (receive P')
-  | dc_cong_close : close $⇛ close
-  | dc_cong_wait : forall P P', P ⇛ P' -> (wait P) $⇛ (wait P')
-  | dc_cong_reflS : forall s, s $⇛ s
-where
-  "s '$⇛' r" := (directed_congruence_statement s r). *)
-
 Inductive directed_congruence : process -> process -> Prop :=
   (* links *)
   | dc_cong_link : forall ml1 ml2 mr1 mr2,
@@ -120,66 +47,21 @@ Inductive directed_congruence : process -> process -> Prop :=
       ml1 !⇛ ml2 -> mr1 !⇛ mr2 -> (link ml1 mr1) ⇛ (link mr2 ml2)
 
   (* cuts *)
-  | dc_cut_comm : forall P P' Q Q', 
-      P ⇛ P' -> Q ⇛ Q' -> (cut P Q) ⇛ (cut Q' P')
-  | dc_cut_assoc_l1 : forall P P' P'' Q Q' R R' R'' L L',
-      (* i don't like the L ⇛ (cut P Q) premise, can we cut it? *)
-      L ⇛ (cut P Q) -> ~ (1 ∈ P) -> P ⇛ P' -> R ⇛ R' ->
-      P'' = down (rename_process P' swap01) ->
-      Q' = rename_process Q swap01 ->
-      R'' = rename_process (up R') swap01 ->
-      (cut Q' R'') ⇛ L' ->
-      (cut L R) ⇛ (cut P'' L')
-  | dc_cut_assoc_l2 : forall P P' P'' Q Q' R R' R'' L L',
-      L ⇛ (cut Q P) -> ~ (1 ∈ P) -> P ⇛ P' -> R ⇛ R' ->
-      P'' = down (rename_process P' swap01) ->
-      Q' = rename_process Q swap01 ->
-      R'' = rename_process (up R') swap01 ->
-      (cut R'' Q') ⇛ L' ->
-      (cut L R) ⇛ (cut P'' L')
-  | dc_cut_assoc_l1_comm : forall P P' P'' Q Q' R R' R'' L L',
-      L ⇛ (cut P Q) -> ~ (1 ∈ P) -> P ⇛ P' -> R ⇛ R' ->
-      P'' = down (rename_process P' swap01) ->
-      Q' = rename_process Q swap01 ->
-      R'' = rename_process (up R') swap01 ->
-      (cut Q' R'') ⇛ L' ->
-      (cut L R) ⇛ (cut L' P'')
-  | dc_cut_assoc_l2_comm : forall P P' P'' Q Q' R R' R'' L L',
-      L ⇛ (cut Q P) -> ~ (1 ∈ P) -> P ⇛ P' -> R ⇛ R' ->
-      P'' = down (rename_process P' swap01) ->
-      Q' = rename_process Q swap01 ->
-      R'' = rename_process (up R') swap01 ->
-      (cut R'' Q') ⇛ L' ->
-      (cut L R) ⇛ (cut L' P'')
-  (* these rules are necessary to ensure admissibility of symmetry *)
-  | dc_cut_assoc_r1 : forall P P' P'' Q Q' R R' R'' L L',
-      L ⇛ (cut Q R) -> ~ (1 ∈ R) -> P ⇛ P' -> R ⇛ R' ->
-      P'' = rename_process (up P') swap01 ->
-      Q' = rename_process Q swap01 ->
-      R'' = down (rename_process R' swap01) ->
-      (cut P'' Q') ⇛ L' ->
-      (cut P L) ⇛ (cut L' R'')
-  | dc_cut_assoc_r2 : forall P P' P'' Q Q' R R' R'' L L',
-      L ⇛ (cut R Q) -> ~ (1 ∈ R) -> P ⇛ P' -> R ⇛ R' ->
-      P'' = rename_process (up P') swap01 ->
-      Q' = rename_process Q swap01 ->
-      R'' = down (rename_process R' swap01) ->
-      (cut Q' P'') ⇛ L' ->
-      (cut P L) ⇛ (cut L' R'')
-  | dc_cut_assoc_r1_comm : forall P P' P'' Q Q' R R' R'' L L',
-      L ⇛ (cut Q R) -> ~ (1 ∈ R) -> P ⇛ P' -> R ⇛ R' ->
-      P'' = rename_process (up P') swap01 ->
-      Q' = rename_process Q swap01 ->
-      R'' = down (rename_process R' swap01) ->
-      (cut P'' Q') ⇛ L' ->
-      (cut P L) ⇛ (cut R'' L')
-  | dc_cut_assoc_r2_comm : forall P P' P'' Q Q' R R' R'' L L',
-      L ⇛ (cut R Q) -> ~ (1 ∈ R) -> P ⇛ P' -> R ⇛ R' ->
-      P'' = rename_process (up P') swap01 ->
-      Q' = rename_process Q swap01 ->
-      R'' = down (rename_process R' swap01) ->
-      (cut Q' P'') ⇛ L' ->
-      (cut P L) ⇛ (cut R'' L')
+  | dc_cut_comm : forall P P' Q Q', P ⇛ P' -> Q ⇛ Q' -> (cut P Q) ⇛ (cut Q' P')
+  | dc_cut_assoc_l : forall P Q R P1 Q1 R1 P' Q' R',
+      ~ (1 ∈ P) ->
+      P ⇛ P1 -> Q ⇛ Q1 -> R ⇛ R1 ->
+      P' = down (rename_process P1 swap01) ->
+      Q' = rename_process Q1 swap01 ->
+      R' = rename_process (up R1) swap01 ->
+      (cut (cut P Q) R) ⇛ (cut P' (cut Q' R'))
+  | dc_cut_assoc_r : forall P Q R P1 Q1 R1 P' Q' R',
+      ~ (1 ∈ R) ->
+      P ⇛ P1 -> Q ⇛ Q1 -> R ⇛ R1 ->
+      P' = rename_process (up P1) swap01 ->
+      Q' = rename_process Q1 swap01 ->
+      R' = down (rename_process R1 swap01) ->
+      (cut P (cut Q R)) ⇛ (cut (cut P' Q') R')
   | dc_cong_cut : forall P P' Q Q', P ⇛ P' -> Q ⇛ Q' -> (cut P Q) ⇛ (cut P' Q')
 
   (* seqs *)
@@ -236,100 +118,6 @@ Proof.
   + econstructor.
 Qed.
 
-(* test *)
-Lemma directed_cong_triangle :
-  (forall P1 P2, P1 ⇛ P2 -> forall P3, P1 ⇛ P3 -> P2 ⇛ P3) /\
-  (forall M1 M2, M1 !⇛ M2 -> forall M3, M1 !⇛ M3 -> M2 !⇛ M3) /\
-  (forall s1 s2, s1 $⇛ s2 -> forall s3, s1 $⇛ s3 -> s2 $⇛ s3).
-Proof.
-  apply directed_cong_ind; intros.
-  + inversion H1; subst.
-    - apply dc_cong_link; try apply H; try apply H0; auto.
-    - apply dc_link; try apply H; try apply H0; auto.
-  + inversion H1; subst.
-    - apply dc_link; try apply H; try apply H0; auto.
-    - apply dc_cong_link; try apply H; try apply H0; auto.
-  + admit.
-  + inversion H3; subst.
-    - assert ( L' ⇛ (cut (rename_process Q swap01) (rename_process (up R) swap01)))
-        by admit.
-      eapply dc_cut_assoc_r1_comm.
-      * apply H4.
-      * admit.
-      * assert (
-          (down (rename_process P' swap01)) ⇛ (down (rename_process P swap01))
-        ) by admit.
-        apply H5.
-      * assert (
-          (rename_process (up R) swap01) ⇛ (rename_process (up Q'0) swap01)
-        ) by admit.
-        apply H5.
-      * autorewrite with up_down_rename_rewrites; auto.
-        admit.
-      * autorewrite with up_down_rename_rewrites. auto.
-      * autorewrite with up_down_rename_rewrites. auto.
-      * apply (H _ H6).
-    - admit.
-    - admit.
-    - 
-Admitted.
-(* test end *)
-
-(******************************************************************************)
-(* Directed congruence is invariant under substitution                        *)
-(******************************************************************************)
-(* Lemma directed_cong_substitution :
-  (forall P Q, P ⇛ Q -> forall σ1 σ2, (forall i, (σ1 i) !⇛ (σ2 i))
-    -> (subst_process P σ1) ⇛ (subst_process Q σ2)) /\
-  (forall M N, M !⇛ N -> forall σ1 σ2, (forall i, (σ1 i) !⇛ (σ2 i))
-    -> (subst_message M σ1) !⇛ (subst_message N σ2)) /\
-  (forall s t, s $⇛ t -> forall σ1 σ2, (forall i, (σ1 i) !⇛ (σ2 i))
-    -> (subst_statement s σ1) $⇛ (subst_statement t σ2)).
-Proof.
-  apply directed_cong_ind; intros; simpl.
-  + admit.
-  + econstructor; try apply H; try apply H0; auto.
-  + admit.
-  + (* up_subst twice results in up in every σ1 i -> ~ 1 ∈ P ...
-       since (up_subst (up_subst σ1)) is id up to index 2, at swap01 is
-       id starting at 2 we can swap rename and subst
-       what remains:
-        down (subst P (up_subst (up_subst σ1)))
-        =  subst (down P) (up_subst σ1)
-        I think the IH is the same as in down_ren_up_ren_commute!?
-
-        We need similar lemmas as below, just with substitution
-       *)
-    admit.
-  + admit.
-  + admit.
-  + admit.
-  + admit.
-Admitted. *)
-
-(* Notes: For ⇛ to be invariant under substitution, we require
-   the congruences from ≡. In this case, reflexivity is derivable so we can drop it.
-
-   Also, the additional premises in the what used to be axiom in ≡ seem
-   redundant now. But idk, we migt still need them later.
-
-   The diamond property immemdiately follows from symmetry but is too weak
-   for parallel reduction: What we need is the following property (pictorally):
-
-        Q                          Q
-     ⇛    ⇛       then         ⇛   ⇛
-    Q1     Q2                  Q1  ⇛  Q2
-
-   With symmetry, this means that we can always convert between diverging
-   congruences in a single step (but now we need additional premises in the axioms).
-   We also need more cut_assoc rules to deal with communication in order to
-   reconciliate in triangle-shape. Note: This also increases the amount of
-   rp_cut_assoc rules (since the link may now occurs in every position).
-
-   Switch back confluence_directed_cong_par_red to
-   forall P Q1 Q2, P ⇛ Q1 -> P ⊵ Q2 -> exists R, Q1 ⊵ R /\ Q2 ⇛ R.
-*)
-
 (******************************************************************************)
 (* Specialized inversion                                                      *)
 (******************************************************************************)
@@ -377,65 +165,22 @@ Lemma directed_cong_in_struct_cong :
   (forall M N, M !⇛ N -> M !≡ N) /\
   (forall s t, s $⇛ t -> s $≡ t).
 Proof.
-  (* apply directed_cong_ind; intros; try (now (econstructor; eauto)).
-  + eapply c_trans. { eapply c_link. }
-    eapply c_cong_link; eauto.
-  + eapply c_trans. { eapply c_cut_comm. }
-    eapply c_cong_cut; eauto.
-  + eapply c_trans. { eapply c_cong_cut. apply H. apply c_refl. }
-    eapply c_trans. { eapply c_cong_cut. eapply c_cong_cut. apply H0. apply c_refl. apply c_refl. }
-    subst. eapply c_trans.
-    - eapply c_cut_assoc; auto. intro Hfv.
-      apply (proj2 ((proj1 free_vars_under_struct_cong) _ _ H0 _)) in Hfv.
-      congruence.
-    - eapply c_cong_cut. apply c_refl. auto.
-      admit.
-  + eapply c_trans. { eapply c_cong_cut. apply H. apply c_refl. }
-    eapply c_trans. { eapply c_cong_cut. eapply c_cong_cut. apply H0. apply c_refl. apply c_refl. }
-    subst. eapply c_trans.
-    - eapply c_cut_assoc; auto. intro Hfv.
-      apply (proj2 ((proj1 free_vars_under_struct_cong) _ _ H0 _)) in Hfv.
-      congruence.
-    - eapply c_trans. apply c_cut_comm. eapply c_cong_cut; try apply c_refl.
-      auto.
-      admit.
-  + eapply c_trans. { eapply c_cong_cut. apply c_refl. apply H. }
-    eapply c_trans. { eapply c_cong_cut. apply c_refl. apply c_cong_cut. apply c_refl. apply H0. }
-    eapply c_comm. eapply c_trans. { eapply c_cong_cut. apply c_comm in H1. apply H1. apply c_refl. }
-    eapply c_trans.
-    - apply c_cut_assoc; auto.
-      assert (~ (0 ∈ (up P))). { apply nfv_lift_n; lia. }
-      replace 1 with (swap01 0) by auto. subst.
-      apply ((proj1 nfv_under_renaming) _ swap01); auto. apply swap01_is_bijective.
-    - subst. autorewrite with up_down_rename_rewrites.
-      * apply c_cong_cut; apply c_refl.
-      * replace 0 with (swap01 1) by auto.
-        apply ((proj1 nfv_under_renaming) _ swap01). apply swap01_is_bijective.
-        intro Hfv. apply (proj2 ((proj1 free_vars_under_struct_cong) _ _ H0 _)) in Hfv.
-        congruence.
-  + eapply c_trans. { eapply c_cong_cut. apply c_refl. apply H. }
-    eapply c_trans. { eapply c_cong_cut. apply c_refl. apply c_cong_cut. apply c_refl. apply H0. }
-    assert ((cut P (cut Q R')) ≡ (cut L' R'')).
-    {
-      eapply c_comm. eapply c_trans. { eapply c_cong_cut. apply c_comm in H1. apply H1. apply c_refl. }
-      eapply c_trans.
-      - apply c_cut_assoc; auto.
-        assert (~ (0 ∈ (up P))). { apply nfv_lift_n; lia. }
-        replace 1 with (swap01 0) by auto. subst.
-        apply ((proj1 nfv_under_renaming) _ swap01); auto. apply swap01_is_bijective.
-      - subst. autorewrite with up_down_rename_rewrites.
-        * apply c_cong_cut; apply c_refl.
-        * replace 0 with (swap01 1) by auto.
-          apply ((proj1 nfv_under_renaming) _ swap01). apply swap01_is_bijective.
-          intro Hfv. apply (proj2 ((proj1 free_vars_under_struct_cong) _ _ H0 _)) in Hfv.
-          congruence.
-    }
-    eapply c_trans. apply H2. apply c_cut_comm.
-  + destruct (proj1 (proj2 struct_cong_d_refl) m).
-    eapply (proj1 (proj2 struct_cong_from_struct_cong_d)); eauto.
-  + destruct (proj2 (proj2 struct_cong_d_refl) s).
-    eapply (proj2 (proj2 struct_cong_from_struct_cong_d)); eauto. *)
-Admitted.
+  apply directed_cong_ind; intros; try (now (econstructor; eauto)).
+  + eapply c_trans. apply c_link. apply c_cong_link; auto.
+  + eapply c_trans. apply c_cut_comm. apply c_cong_cut; auto.
+  + eapply c_trans.
+    - eapply c_cong_cut; eauto. eapply c_cong_cut; eauto.
+    - subst; apply c_cut_assoc; auto. intro Hfv. apply c_comm in H.
+      apply ((proj1 free_vars_under_struct_cong) _ _ H _) in Hfv. congruence.
+  + apply c_comm. eapply c_trans.
+    - eapply c_cut_assoc; auto. rewrite e. apply nfv_10_swap. apply nfv_lift_n; lia.
+    - subst; autorewrite with up_down_rename_rewrites.
+      * apply c_cong_cut. apply c_comm; auto. apply c_cong_cut; apply c_comm; auto.
+      * apply nfv_01_swap. intro Hfv. apply c_comm in H1.
+        apply ((proj1 free_vars_under_struct_cong) _ _ H1 _) in Hfv. congruence.
+  + apply struct_cong_reflM.
+  + apply struct_cong_reflS.
+Qed.
 
 Lemma ren_up_up_ren_commute :
   (forall P, forall r k,
@@ -569,21 +314,50 @@ Lemma directed_cong_invariant_under_renaming :
   /\
   (forall s t, s $⇛ t -> forall r, bijective r -> (rename_statement s r) $⇛ (rename_statement t r)).
 Proof.
-  (* apply directed_cong_ind; intros; try (now (simpl; econstructor; eauto));
+  apply directed_cong_ind; intros; try (now (simpl; econstructor; eauto));
   try (now (simpl; econstructor; try apply H; try apply H0; auto;
        try apply shift_preserves_bijection;try apply shift_preserves_bijection;  auto)).
-  + simpl. eapply dc_cut_assoc_l.
-    - apply H. apply shift_preserves_bijection. auto.
-    - fold rename_process.
-      replace 1 with (up_ren (up_ren r) 1) by auto.
-      apply ((proj1 nfv_under_renaming) _ (up_ren (up_ren r)) _) in n;
-      try (repeat apply shift_preserves_bijection; auto).
-    - fold rename_process. apply H0.
-      repeat apply shift_preserves_bijection. auto.
-    - rewrite e. unfold down.
+  + simpl. subst. eapply dc_cut_assoc_l.
+    - replace 1 with ((up_ren (up_ren r)) 1) by auto. apply nfv_under_renaming; auto.
+      repeat apply shift_preserves_bijection; auto.
+    - apply H; repeat apply shift_preserves_bijection; auto.
+    - apply H0; repeat apply shift_preserves_bijection; auto.
+    - apply H1; repeat apply shift_preserves_bijection; auto.
+    - assert (
+        (rename_process (down (rename_process P1 swap01)) (up_ren r)) =
+        (down (rename_process (rename_process P1 swap01) (up_ren (up_ren r))))
+      ).
+      {
+        unfold down. rewrite <- (proj1 down_ren_up_ren_commute); auto.
+        + apply shift_preserves_bijection; auto.
+        + intros [|[|]] ?; exfalso; lia.
+        + apply nfv_01_swap; auto. intro Hfv. apply directed_cong_in_struct_cong in d.
+          apply c_comm in d. apply ((proj1 free_vars_under_struct_cong) _ _ d) in Hfv; congruence.
+      }
+      rewrite H3.
       assert (
-        rename_process (rename_process P' (up_ren (up_ren r))) swap01 =
-        rename_process (rename_process P' swap01) (up_ren (up_ren r))
+        rename_process (rename_process P1 (up_ren (up_ren r))) swap01 =
+        rename_process (rename_process P1 swap01) (up_ren (up_ren r))
+      ).
+      {
+        rewrite ((proj1 renamings_compose) _ _ _ (Basics.compose swap01 (up_ren (up_ren r)))).
+        rewrite ((proj1 renamings_compose) _ _ _ (Basics.compose swap01 (up_ren (up_ren r)))).
+        reflexivity. all: intros[|[|]]; auto.
+      }
+      rewrite H4. auto.
+    - assert (
+        rename_process (rename_process Q1 (up_ren (up_ren r))) swap01 =
+        rename_process (rename_process Q1 swap01) (up_ren (up_ren r))
+      ).
+      {
+        rewrite ((proj1 renamings_compose) _ _ _ (Basics.compose swap01 (up_ren (up_ren r)))).
+        rewrite ((proj1 renamings_compose) _ _ _ (Basics.compose swap01 (up_ren (up_ren r)))).
+        reflexivity. all: intros[|[|]]; auto.
+      }
+      rewrite H3. auto.
+    - assert (
+        (rename_process (rename_process (up R1) swap01) (up_ren (up_ren r))) =
+        (rename_process (rename_process (up R1) (up_ren (up_ren r))) swap01)
       ).
       {
         rewrite ((proj1 renamings_compose) _ _ _ (Basics.compose swap01 (up_ren (up_ren r)))).
@@ -591,40 +365,9 @@ Proof.
         reflexivity. all: intros[|[|]]; auto.
       }
       rewrite H3.
-      assert (~ 1 ∈ P').
-      {
-        intro Hfv. apply directed_cong_in_struct_cong in d0. apply c_comm in d0.
-        apply ((proj1 free_vars_under_struct_cong) _ _ d0) in Hfv. congruence.
-      }
-      rewrite (proj1 down_ren_up_ren_commute); auto.
-      * apply shift_preserves_bijection; auto.
-      * intros. exfalso; lia.
-      * replace 0 with (swap01 1) by auto. apply nfv_under_renaming; auto.
-        apply swap01_is_bijective.
-    - fold rename_process. auto.
-    - auto.
-    - assert (
-        rename_process (rename_process Q (up_ren (up_ren r))) swap01 =
-        rename_process (rename_process Q swap01) (up_ren (up_ren r))
-      ).
-      {
-        rewrite ((proj1 renamings_compose) _ _ _ (Basics.compose swap01 (up_ren (up_ren r)))).
-        rewrite ((proj1 renamings_compose) _ _ _ (Basics.compose swap01 (up_ren (up_ren r)))).
-        reflexivity. all: intros[|[|]]; auto.
-      }
-      rewrite H3. rewrite <- e0.
       assert (
-        rename_process (rename_process (up R) swap01) (up_ren (up_ren r)) =
-        rename_process (rename_process (up R) (up_ren (up_ren r))) swap01
-      ).
-      {
-        rewrite ((proj1 renamings_compose) _ _ _ (Basics.compose swap01 (up_ren (up_ren r)))).
-        rewrite ((proj1 renamings_compose) _ _ _ (Basics.compose swap01 (up_ren (up_ren r)))).
-        reflexivity. all: intros[|[|]]; auto.
-      }
-      assert (
-        up (rename_process R (up_ren r)) =
-        rename_process (up R) (up_ren (up_ren r))
+        up (rename_process R1 (up_ren r)) =
+        rename_process (up R1) (up_ren (up_ren r))
       ).
       {
         unfold up.
@@ -632,25 +375,43 @@ Proof.
         + apply shift_preserves_bijection; auto.
         + intros. exfalso; lia.
       }
-      rewrite H5. rewrite <- H4. rewrite <- e1.
-      replace
-        (cut (rename_process Q' (up_ren (up_ren r))) (rename_process R' (up_ren (up_ren r))))
-        with
-        (rename_process (cut Q' R') (up_ren r))
-        by auto.
-      apply H1. apply shift_preserves_bijection; auto.
-  + simpl. eapply dc_cut_assoc_l_comm.
-    - apply H. apply shift_preserves_bijection. auto.
-    - fold rename_process.
-      replace 1 with (up_ren (up_ren r) 1) by auto.
-      apply ((proj1 nfv_under_renaming) _ (up_ren (up_ren r)) _) in n;
-      try (repeat apply shift_preserves_bijection; auto).
-    - fold rename_process. apply H0.
-      repeat apply shift_preserves_bijection. auto.
-    - rewrite e. unfold down.
+      rewrite H4. auto.
+  + eapply dc_cut_assoc_r; fold rename_process.
+    - replace 1 with ((up_ren (up_ren r)) 1) by auto.
+      apply nfv_under_renaming; auto. repeat apply shift_preserves_bijection; auto.
+    - apply H. apply shift_preserves_bijection; auto.
+    - apply H0; repeat apply shift_preserves_bijection; auto.
+    - apply H1; repeat apply shift_preserves_bijection; auto.
+    - rewrite e.
       assert (
-        rename_process (rename_process P' (up_ren (up_ren r))) swap01 =
-        rename_process (rename_process P' swap01) (up_ren (up_ren r))
+        rename_process (rename_process (up P1) (up_ren (up_ren r))) swap01 =
+        rename_process (rename_process (up P1) swap01) (up_ren (up_ren r))
+      ).
+      {
+        rewrite ((proj1 renamings_compose) _ _ _ (Basics.compose swap01 (up_ren (up_ren r)))).
+        rewrite ((proj1 renamings_compose) _ _ _ (Basics.compose swap01 (up_ren (up_ren r)))).
+        reflexivity. all: intros[|[|]]; auto.
+      }
+      rewrite <- H3.
+      assert (
+        up (rename_process P1 (up_ren r)) =
+        rename_process (up P1) (up_ren (up_ren r))
+      ).
+      {
+        unfold up.
+        rewrite (proj1 ren_up_up_ren_commute); auto.
+        + apply shift_preserves_bijection; auto.
+        + intros. exfalso; lia.
+      }
+      rewrite H4. auto.
+    - rewrite e0.
+      rewrite ((proj1 renamings_compose) _ _ _ (Basics.compose swap01 (up_ren (up_ren r)))).
+      rewrite ((proj1 renamings_compose) _ _ _ (Basics.compose swap01 (up_ren (up_ren r)))).
+      reflexivity. all: intros[|[|]]; auto.
+    - rewrite e1.
+      assert (
+        rename_process (rename_process R1 (up_ren (up_ren r))) swap01 =
+        rename_process (rename_process R1 swap01) (up_ren (up_ren r))
       ).
       {
         rewrite ((proj1 renamings_compose) _ _ _ (Basics.compose swap01 (up_ren (up_ren r)))).
@@ -658,189 +419,19 @@ Proof.
         reflexivity. all: intros[|[|]]; auto.
       }
       rewrite H3.
-      assert (~ 1 ∈ P').
-      {
-        intro Hfv. apply directed_cong_in_struct_cong in d0. apply c_comm in d0.
-        apply ((proj1 free_vars_under_struct_cong) _ _ d0) in Hfv. congruence.
-      }
-      rewrite (proj1 down_ren_up_ren_commute); auto.
-      * apply shift_preserves_bijection; auto.
-      * intros. exfalso; lia.
-      * replace 0 with (swap01 1) by auto. apply nfv_under_renaming; auto.
-        apply swap01_is_bijective.
-    - fold rename_process. auto.
-    - auto.
-    - assert (
-        rename_process (rename_process Q (up_ren (up_ren r))) swap01 =
-        rename_process (rename_process Q swap01) (up_ren (up_ren r))
-      ).
-      {
-        rewrite ((proj1 renamings_compose) _ _ _ (Basics.compose swap01 (up_ren (up_ren r)))).
-        rewrite ((proj1 renamings_compose) _ _ _ (Basics.compose swap01 (up_ren (up_ren r)))).
-        reflexivity. all: intros[|[|]]; auto.
-      }
-      rewrite H3. rewrite <- e0.
       assert (
-        rename_process (rename_process (up R) swap01) (up_ren (up_ren r)) =
-        rename_process (rename_process (up R) (up_ren (up_ren r))) swap01
+        (rename_process (down (rename_process R1 swap01)) (up_ren r)) =
+        (down (rename_process (rename_process R1 swap01) (up_ren (up_ren r))))
       ).
       {
-        rewrite ((proj1 renamings_compose) _ _ _ (Basics.compose swap01 (up_ren (up_ren r)))).
-        rewrite ((proj1 renamings_compose) _ _ _ (Basics.compose swap01 (up_ren (up_ren r)))).
-        reflexivity. all: intros[|[|]]; auto.
-      }
-      assert (
-        up (rename_process R (up_ren r)) =
-        rename_process (up R) (up_ren (up_ren r))
-      ).
-      {
-        unfold up.
-        rewrite (proj1 ren_up_up_ren_commute); auto.
+        unfold down. rewrite <- (proj1 down_ren_up_ren_commute); auto.
         + apply shift_preserves_bijection; auto.
-        + intros. exfalso; lia.
+        + intros [|[|]] ?; exfalso; lia.
+        + apply nfv_01_swap; auto. intro Hfv. apply directed_cong_in_struct_cong in d1.
+          apply c_comm in d1. apply ((proj1 free_vars_under_struct_cong) _ _ d1) in Hfv; congruence.
       }
-      rewrite H5. rewrite <- H4. rewrite <- e1.
-      replace
-        (cut (rename_process Q' (up_ren (up_ren r))) (rename_process R' (up_ren (up_ren r))))
-        with
-        (rename_process (cut Q' R') (up_ren r))
-        by auto.
-      apply H1. apply shift_preserves_bijection; auto.
-  + simpl. eapply dc_cut_assoc_r.
-    - apply H. apply shift_preserves_bijection. auto.
-    - fold rename_process.
-      replace 1 with (up_ren (up_ren r) 1) by auto.
-      apply ((proj1 nfv_under_renaming) _ (up_ren (up_ren r)) _) in n;
-      try (repeat apply shift_preserves_bijection; auto).
-    - fold rename_process. apply H0.
-      repeat apply shift_preserves_bijection. auto.
-    - auto.
-    - fold rename_process. auto.
-    - rewrite e1. unfold down.
-      assert (
-        rename_process (rename_process R' (up_ren (up_ren r))) swap01 =
-        rename_process (rename_process R' swap01) (up_ren (up_ren r))
-      ).
-      {
-        rewrite ((proj1 renamings_compose) _ _ _ (Basics.compose swap01 (up_ren (up_ren r)))).
-        rewrite ((proj1 renamings_compose) _ _ _ (Basics.compose swap01 (up_ren (up_ren r)))).
-        reflexivity. all: intros[|[|]]; auto.
-      }
-      rewrite H3.
-      assert (~ 1 ∈ R').
-      {
-        intro Hfv. apply directed_cong_in_struct_cong in d0. apply c_comm in d0.
-        apply ((proj1 free_vars_under_struct_cong) _ _ d0) in Hfv. congruence.
-      }
-      rewrite (proj1 down_ren_up_ren_commute); auto.
-      * apply shift_preserves_bijection; auto.
-      * intros. exfalso; lia.
-      * replace 0 with (swap01 1) by auto. apply nfv_under_renaming; auto.
-        apply swap01_is_bijective.
-    - assert (
-        rename_process (rename_process Q (up_ren (up_ren r))) swap01 =
-        rename_process (rename_process Q swap01) (up_ren (up_ren r))
-      ).
-      {
-        rewrite ((proj1 renamings_compose) _ _ _ (Basics.compose swap01 (up_ren (up_ren r)))).
-        rewrite ((proj1 renamings_compose) _ _ _ (Basics.compose swap01 (up_ren (up_ren r)))).
-        reflexivity. all: intros[|[|]]; auto.
-      }
-      rewrite H3. rewrite <- e0.
-      assert (
-        rename_process (rename_process (up P) swap01) (up_ren (up_ren r)) =
-        rename_process (rename_process (up P) (up_ren (up_ren r))) swap01
-      ).
-      {
-        rewrite ((proj1 renamings_compose) _ _ _ (Basics.compose swap01 (up_ren (up_ren r)))).
-        rewrite ((proj1 renamings_compose) _ _ _ (Basics.compose swap01 (up_ren (up_ren r)))).
-        reflexivity. all: intros[|[|]]; auto.
-      }
-      assert (
-        up (rename_process P (up_ren r)) =
-        rename_process (up P) (up_ren (up_ren r))
-      ).
-      {
-        unfold up.
-        rewrite (proj1 ren_up_up_ren_commute); auto.
-        + apply shift_preserves_bijection; auto.
-        + intros. exfalso; lia.
-      }
-      rewrite H5. rewrite <- H4. rewrite <- e.
-      replace
-        (cut (rename_process P' (up_ren (up_ren r))) (rename_process Q' (up_ren (up_ren r))))
-        with
-        (rename_process (cut P' Q') (up_ren r))
-        by auto.
-      apply H1. apply shift_preserves_bijection; auto.
-  + simpl. eapply dc_cut_assoc_r_comm.
-    - apply H. apply shift_preserves_bijection. auto.
-    - fold rename_process.
-      replace 1 with (up_ren (up_ren r) 1) by auto.
-      apply ((proj1 nfv_under_renaming) _ (up_ren (up_ren r)) _) in n;
-      try (repeat apply shift_preserves_bijection; auto).
-    - fold rename_process. apply H0.
-      repeat apply shift_preserves_bijection. auto.
-    - auto.
-    - fold rename_process. auto.
-    - rewrite e1. unfold down.
-      assert (
-        rename_process (rename_process R' (up_ren (up_ren r))) swap01 =
-        rename_process (rename_process R' swap01) (up_ren (up_ren r))
-      ).
-      {
-        rewrite ((proj1 renamings_compose) _ _ _ (Basics.compose swap01 (up_ren (up_ren r)))).
-        rewrite ((proj1 renamings_compose) _ _ _ (Basics.compose swap01 (up_ren (up_ren r)))).
-        reflexivity. all: intros[|[|]]; auto.
-      }
-      rewrite H3.
-      assert (~ 1 ∈ R').
-      {
-        intro Hfv. apply directed_cong_in_struct_cong in d0. apply c_comm in d0.
-        apply ((proj1 free_vars_under_struct_cong) _ _ d0) in Hfv. congruence.
-      }
-      rewrite (proj1 down_ren_up_ren_commute); auto.
-      * apply shift_preserves_bijection; auto.
-      * intros. exfalso; lia.
-      * replace 0 with (swap01 1) by auto. apply nfv_under_renaming; auto.
-        apply swap01_is_bijective.
-    - assert (
-        rename_process (rename_process Q (up_ren (up_ren r))) swap01 =
-        rename_process (rename_process Q swap01) (up_ren (up_ren r))
-      ).
-      {
-        rewrite ((proj1 renamings_compose) _ _ _ (Basics.compose swap01 (up_ren (up_ren r)))).
-        rewrite ((proj1 renamings_compose) _ _ _ (Basics.compose swap01 (up_ren (up_ren r)))).
-        reflexivity. all: intros[|[|]]; auto.
-      }
-      rewrite H3. rewrite <- e0.
-      assert (
-        rename_process (rename_process (up P) swap01) (up_ren (up_ren r)) =
-        rename_process (rename_process (up P) (up_ren (up_ren r))) swap01
-      ).
-      {
-        rewrite ((proj1 renamings_compose) _ _ _ (Basics.compose swap01 (up_ren (up_ren r)))).
-        rewrite ((proj1 renamings_compose) _ _ _ (Basics.compose swap01 (up_ren (up_ren r)))).
-        reflexivity. all: intros[|[|]]; auto.
-      }
-      assert (
-        up (rename_process P (up_ren r)) =
-        rename_process (up P) (up_ren (up_ren r))
-      ).
-      {
-        unfold up.
-        rewrite (proj1 ren_up_up_ren_commute); auto.
-        + apply shift_preserves_bijection; auto.
-        + intros. exfalso; lia.
-      }
-      rewrite H5. rewrite <- H4. rewrite <- e.
-      replace
-        (cut (rename_process P' (up_ren (up_ren r))) (rename_process Q' (up_ren (up_ren r))))
-        with
-        (rename_process (cut P' Q') (up_ren r))
-        by auto.
-      apply H1. apply shift_preserves_bijection; auto. *)
-Admitted.
+      rewrite H4. auto.
+Qed.
 
 Lemma lift_after_down_lt_commute :
   (forall P,
@@ -1085,96 +676,36 @@ Lemma directed_cong_invariant_under_upshifting :
   (forall M N, M !⇛ N -> forall k, (lift_message M k 1) !⇛ (lift_message N k 1)) /\
   (forall s t, s $⇛ t -> forall k, (lift_statement s k 1) $⇛ (lift_statement t k 1)).
 Proof.
-  (* apply directed_cong_ind; intros; try now (econstructor; eauto).
-  + simpl. subst. eapply dc_cut_assoc_l.
+  apply directed_cong_ind; intros; try now (econstructor; eauto).
+  + simpl; subst. eapply dc_cut_assoc_l.
+    - apply nfv_up_lt; auto; lia.
     - apply H.
-    - fold lift_process. apply nfv_up_lt; try lia. auto.
-    - fold lift_process. apply H0.
-    - unfold down.
-      rewrite (proj1 lift_after_down_lt_commute); try lia.
-      rewrite (proj1 lift_at_k_rename_id_after_k_commute); auto. apply swap01_is_bijective.
-      intros [|[|]] ?; auto; exfalso; lia.
-    - auto.
-    - auto.
-    - fold lift_process.
-      rewrite <- (proj1 lift_at_k_rename_id_after_k_commute); try apply swap01_is_bijective.
-      unfold up. rewrite <- (proj1 lift_k_lift_Sj_lt_commute); try lia.
-      rewrite <- (proj1 lift_at_k_rename_id_after_k_commute); try apply swap01_is_bijective.
-      replace (
-        (cut (lift_process (rename_process Q swap01) (S (S k)) 1)
-             (lift_process (rename_process (lift_process R 0 1) swap01) (S (S k)) 1))
-      ) with (
-        (lift_process (cut (rename_process Q swap01) (rename_process (up R) swap01)) (S k) 1)
-      ) by auto.
-      apply H1.
-      all: intros [|[|]] ?; auto; exfalso; lia.
-  + simpl. subst. eapply dc_cut_assoc_l_comm.
-    - apply H.
-    - fold lift_process. apply nfv_up_lt; try lia. auto.
-    - fold lift_process. apply H0.
-    - unfold down.
-      rewrite (proj1 lift_after_down_lt_commute); try lia.
-      rewrite (proj1 lift_at_k_rename_id_after_k_commute); auto. apply swap01_is_bijective.
-      intros [|[|]] ?; auto; exfalso; lia.
-    - auto.
-    - auto.
-    - fold lift_process.
-      rewrite <- (proj1 lift_at_k_rename_id_after_k_commute); try apply swap01_is_bijective.
-      unfold up. rewrite <- (proj1 lift_k_lift_Sj_lt_commute); try lia.
-      rewrite <- (proj1 lift_at_k_rename_id_after_k_commute); try apply swap01_is_bijective.
-      replace (
-        (cut (lift_process (rename_process Q swap01) (S (S k)) 1)
-             (lift_process (rename_process (lift_process R 0 1) swap01) (S (S k)) 1))
-      ) with (
-        (lift_process (cut (rename_process Q swap01) (rename_process (up R) swap01)) (S k) 1)
-      ) by auto.
-      apply H1.
-      all: intros [|[|]] ?; auto; exfalso; lia.
-  + simpl. subst. eapply dc_cut_assoc_r.
-    - apply H.
-    - apply nfv_up_lt; try lia. auto.
     - apply H0.
-    - auto.
-    - fold lift_process. auto.
+    - apply H1.
     - unfold down.
       rewrite (proj1 lift_after_down_lt_commute); try lia.
       rewrite (proj1 lift_at_k_rename_id_after_k_commute); auto. apply swap01_is_bijective.
       intros [|[|]] ?; auto; exfalso; lia.
-    - fold lift_process.
-      rewrite <- (proj1 lift_at_k_rename_id_after_k_commute); try apply swap01_is_bijective.
-      unfold up. rewrite <- (proj1 lift_k_lift_Sj_lt_commute); try lia.
-      rewrite <- (proj1 lift_at_k_rename_id_after_k_commute); try apply swap01_is_bijective.
-      replace (
-        (cut (lift_process (rename_process Q swap01) (S (S k)) 1)
-             (lift_process (rename_process (lift_process R 0 1) swap01) (S (S k)) 1))
-      ) with (
-        (lift_process (cut (rename_process Q swap01) (rename_process (up R) swap01)) (S k) 1)
-      ) by auto.
-      apply H1.
-      all: intros [|[|]] ?; auto; exfalso; lia.
-  + simpl. subst. eapply dc_cut_assoc_r_comm.
+    - rewrite <- (proj1 lift_at_k_rename_id_after_k_commute); auto; try apply swap01_is_bijective.
+      intros [|[|]] ?; auto; exfalso; lia.
+    - unfold up. rewrite <- (proj1 lift_k_lift_Sj_lt_commute); try lia.
+      rewrite (proj1 lift_at_k_rename_id_after_k_commute); try apply swap01_is_bijective; auto.
+      intros [|[|]] ?; auto; exfalso; lia.
+  + simpl; subst. eapply dc_cut_assoc_r.
+    - apply nfv_up_lt; auto; lia.
     - apply H.
-    - apply nfv_up_lt; try lia. auto.
     - apply H0.
-    - auto.
-    - fold lift_process. auto.
+    - apply H1.
+    - unfold up. rewrite <- (proj1 lift_k_lift_Sj_lt_commute); try lia.
+      rewrite (proj1 lift_at_k_rename_id_after_k_commute); try apply swap01_is_bijective; auto.
+      intros [|[|]] ?; auto; exfalso; lia.
+    - rewrite <- (proj1 lift_at_k_rename_id_after_k_commute); auto; try apply swap01_is_bijective.
+      intros [|[|]] ?; auto; exfalso; lia.
     - unfold down.
       rewrite (proj1 lift_after_down_lt_commute); try lia.
       rewrite (proj1 lift_at_k_rename_id_after_k_commute); auto. apply swap01_is_bijective.
       intros [|[|]] ?; auto; exfalso; lia.
-    - fold lift_process.
-      rewrite <- (proj1 lift_at_k_rename_id_after_k_commute); try apply swap01_is_bijective.
-      unfold up. rewrite <- (proj1 lift_k_lift_Sj_lt_commute); try lia.
-      rewrite <- (proj1 lift_at_k_rename_id_after_k_commute); try apply swap01_is_bijective.
-      replace (
-        (cut (lift_process (rename_process Q swap01) (S (S k)) 1)
-             (lift_process (rename_process (lift_process R 0 1) swap01) (S (S k)) 1))
-      ) with (
-        (lift_process (cut (rename_process Q swap01) (rename_process (up R) swap01)) (S k) 1)
-      ) by auto.
-      apply H1.
-      all: intros [|[|]] ?; auto; exfalso; lia. *)
-Admitted.
+Qed.
 
 Lemma directed_cong_invariant_under_downshifting :
   (forall P Q, P ⇛ Q -> forall k,
@@ -1184,7 +715,7 @@ Lemma directed_cong_invariant_under_downshifting :
   (forall s t, s $⇛ t -> forall k,
     (~ (occurs_free_statement k s)) -> ((down1_statement s k) $⇛ (down1_statement t k))).
 Proof.
-  (* apply directed_cong_ind; intros; simpl; try (now (econstructor));
+  apply directed_cong_ind; intros; simpl; try (now (econstructor));
   try match goal with
   | [ IH1 : forall _, ~ _ -> (down1_message ?ml1 _) !⇛ (down1_message ?ml2 _),
       IH2 : forall _, ~ _ -> (down1_message ?mr1 _) !⇛ (down1_message ?mr2 _),
@@ -1203,290 +734,50 @@ Proof.
       |- _ ]
     => econstructor; try apply (IH1 (S k)); try apply IH1; intro Hfv; apply H; free_var_econstructor; auto
   end.
-  + eapply dc_cut_assoc_l.
-    - apply H. intros Hfv. apply H2. repeat free_var_econstructor; eauto.
-    - fold down1_process. apply (proj1 nfv_down_lt); auto. lia.
-    - fold down1_process. apply H0.
-      intro Hfv. apply H2. apply fv_cut_l.
-      apply directed_cong_in_struct_cong in d.
-      assert ((S k) ∈ (cut P Q)) by (repeat free_var_econstructor; eauto).
-      apply ((proj1 free_vars_under_struct_cong) _ _ d) in H3. auto.
-    - subst. unfold down.
-      rewrite <- (proj1 down_at_k_rename_id_after_k_commute).
-      * rewrite (proj1 down_k_down_Sj_lt_commute); auto. lia.
-      * apply swap01_is_bijective.
-      * intros [|[|]] ?; auto; exfalso; lia.
-    - fold down1_process. auto.
-    - auto.
-    - fold lift_process.
+  + eapply dc_cut_assoc_l; subst.
+    - apply nfv_down_lt; auto; lia.
+    - apply H. intro Hfv. apply H2. repeat free_var_econstructor; auto.
+    - apply H0. intro Hfv. apply H2. repeat free_var_econstructor; auto.
+    - apply H1. intro Hfv. apply H2. repeat free_var_econstructor; auto.
+    - unfold down.
       rewrite <- (proj1 down_at_k_rename_id_after_k_commute); try apply swap01_is_bijective.
-      rewrite <- e0.
-      unfold up.
-      rewrite <- (proj1 down_after_down_gt_commute); try lia.
+      rewrite (proj1 down_k_down_Sj_lt_commute); auto; try lia.
+      intros [|[|]] ?; auto; exfalso; lia.
+    - rewrite <- (proj1 down_at_k_rename_id_after_k_commute); auto; try apply swap01_is_bijective.
+      intros [|[|]] ?; auto; exfalso; lia.
+    - unfold up.
+      rewrite (proj1 down_at_k_rename_id_after_k_commute); try apply swap01_is_bijective.
+      rewrite <- (proj1 down_after_down_gt_commute); try lia. auto.
+      intros [|[|]] ?; eauto; exfalso; lia.
+  + eapply dc_cut_assoc_r; subst.
+    - apply nfv_down_lt; auto; lia.
+    - apply H. intro Hfv. apply H2. repeat free_var_econstructor; auto.
+    - apply H0. intro Hfv. apply H2. apply fv_cut_r. free_var_econstructor; auto.
+    - apply H1. intro Hfv. apply H2. apply fv_cut_r; apply fv_cut_r; auto.
+    - unfold up.
+      rewrite (proj1 down_at_k_rename_id_after_k_commute); try apply swap01_is_bijective.
+      rewrite <- (proj1 down_after_down_gt_commute); try lia. auto.
+      intros [|[|]] ?; eauto; exfalso; lia.
+    - rewrite <- (proj1 down_at_k_rename_id_after_k_commute); auto; try apply swap01_is_bijective.
+      intros [|[|]] ?; auto; exfalso; lia.
+    - unfold down.
       rewrite <- (proj1 down_at_k_rename_id_after_k_commute); try apply swap01_is_bijective.
-      replace (lift_process R 0 1) with (up R) by auto. rewrite <- e1.
-      apply H1.
-      * intro Hfv. inversion Hfv; subst.
-        ++ replace (S (S k)) with (swap01 (S (S k))) in H5 by auto.
-           apply fv_under_renaming in H5; try apply swap01_is_bijective.
-           apply H2. apply fv_cut_l.
-           apply directed_cong_in_struct_cong in d.
-           assert ((S k) ∈ (cut P Q)) by (repeat free_var_econstructor; eauto).
-           apply ((proj1 free_vars_under_struct_cong) _ _ d) in H3. auto.
-        ++ apply H2. apply fv_cut_r.
-           replace (S (S k)) with (swap01 (S (S k))) in H5 by auto.
-           apply fv_under_renaming in H5; try apply swap01_is_bijective.
-           apply fv_up_Sn2 in H5; auto; lia.
-      * intros [|[|]] ?; auto; exfalso; lia.
-      * intros [|[|]] ?; auto; exfalso; lia.
-  + eapply dc_cut_assoc_l_comm.
-    - apply H. intros Hfv. apply H2. repeat free_var_econstructor; eauto.
-    - fold down1_process. apply (proj1 nfv_down_lt); auto. lia.
-    - fold down1_process. apply H0.
-      intro Hfv. apply H2. apply fv_cut_l.
-      apply directed_cong_in_struct_cong in d.
-      assert ((S k) ∈ (cut P Q)) by (repeat free_var_econstructor; eauto).
-      apply ((proj1 free_vars_under_struct_cong) _ _ d) in H3. auto.
-    - subst. unfold down.
-      rewrite <- (proj1 down_at_k_rename_id_after_k_commute).
-      * rewrite (proj1 down_k_down_Sj_lt_commute); auto. lia.
-      * apply swap01_is_bijective.
-      * intros [|[|]] ?; auto; exfalso; lia.
-    - fold down1_process. auto.
-    - auto.
-    - fold lift_process.
-      rewrite <- (proj1 down_at_k_rename_id_after_k_commute); try apply swap01_is_bijective.
-      rewrite <- e0.
-      unfold up.
-      rewrite <- (proj1 down_after_down_gt_commute); try lia.
-      rewrite <- (proj1 down_at_k_rename_id_after_k_commute); try apply swap01_is_bijective.
-      replace (lift_process R 0 1) with (up R) by auto. rewrite <- e1.
-      apply H1.
-      * intro Hfv. inversion Hfv; subst.
-        ++ replace (S (S k)) with (swap01 (S (S k))) in H5 by auto.
-           apply fv_under_renaming in H5; try apply swap01_is_bijective.
-           apply H2. apply fv_cut_l.
-           apply directed_cong_in_struct_cong in d.
-           assert ((S k) ∈ (cut P Q)) by (repeat free_var_econstructor; eauto).
-           apply ((proj1 free_vars_under_struct_cong) _ _ d) in H3. auto.
-        ++ apply H2. apply fv_cut_r.
-           replace (S (S k)) with (swap01 (S (S k))) in H5 by auto.
-           apply fv_under_renaming in H5; try apply swap01_is_bijective.
-           apply fv_up_Sn2 in H5; auto; lia.
-      * intros [|[|]] ?; auto; exfalso; lia.
-      * intros [|[|]] ?; auto; exfalso; lia.
-  + eapply dc_cut_assoc_r.
-    - apply H. intros Hfv. apply H2. repeat free_var_econstructor; eauto.
-    - fold down1_process. apply (proj1 nfv_down_lt); auto. lia.
-    - fold down1_process. apply H0.
-      intro Hfv. apply H2. apply fv_cut_r.
-      apply directed_cong_in_struct_cong in d.
-      assert ((S k) ∈ (cut Q R)) by (repeat free_var_econstructor; eauto).
-      apply ((proj1 free_vars_under_struct_cong) _ _ d) in H3. auto.
-    - auto.
-    - fold down1_process. auto.
-    - subst. unfold down.
-      rewrite <- (proj1 down_at_k_rename_id_after_k_commute).
-      * rewrite (proj1 down_k_down_Sj_lt_commute); auto. lia.
-      * apply swap01_is_bijective.
-      * intros [|[|]] ?; auto; exfalso; lia.
-    - fold lift_process.
-      rewrite <- (proj1 down_at_k_rename_id_after_k_commute); try apply swap01_is_bijective.
-      rewrite <- e0.
-      unfold up.
-      rewrite <- (proj1 down_after_down_gt_commute); try lia.
-      rewrite <- (proj1 down_at_k_rename_id_after_k_commute); try apply swap01_is_bijective.
-      replace (lift_process P 0 1) with (up P) by auto. rewrite <- e.
-      apply H1.
-      * intro Hfv. inversion Hfv; subst.
-        ++ replace (S (S k)) with (swap01 (S (S k))) in H5 by auto.
-           apply fv_under_renaming in H5; try apply swap01_is_bijective.
-           apply H2. apply fv_cut_l.
-           apply fv_up_Sn2 in H5; auto; lia.
-        ++ apply H2. apply fv_cut_r.
-           replace (S (S k)) with (swap01 (S (S k))) in H5 by auto.
-           apply fv_under_renaming in H5; try apply swap01_is_bijective.
-           apply directed_cong_in_struct_cong in d.
-           assert ((S k) ∈ (cut Q R)) by (repeat free_var_econstructor; eauto).
-           apply ((proj1 free_vars_under_struct_cong) _ _ d) in H3. auto.
-      * intros [|[|]] ?; auto; exfalso; lia.
-      * intros [|[|]] ?; auto; exfalso; lia.
-  + eapply dc_cut_assoc_r_comm.
-    - apply H. intros Hfv. apply H2. repeat free_var_econstructor; eauto.
-    - fold down1_process. apply (proj1 nfv_down_lt); auto. lia.
-    - fold down1_process. apply H0.
-      intro Hfv. apply H2. apply fv_cut_r.
-      apply directed_cong_in_struct_cong in d.
-      assert ((S k) ∈ (cut Q R)) by (repeat free_var_econstructor; eauto).
-      apply ((proj1 free_vars_under_struct_cong) _ _ d) in H3. auto.
-    - auto.
-    - fold down1_process. auto.
-    - subst. unfold down.
-      rewrite <- (proj1 down_at_k_rename_id_after_k_commute).
-      * rewrite (proj1 down_k_down_Sj_lt_commute); auto. lia.
-      * apply swap01_is_bijective.
-      * intros [|[|]] ?; auto; exfalso; lia.
-    - fold lift_process.
-      rewrite <- (proj1 down_at_k_rename_id_after_k_commute); try apply swap01_is_bijective.
-      rewrite <- e0.
-      unfold up.
-      rewrite <- (proj1 down_after_down_gt_commute); try lia.
-      rewrite <- (proj1 down_at_k_rename_id_after_k_commute); try apply swap01_is_bijective.
-      replace (lift_process P 0 1) with (up P) by auto. rewrite <- e.
-      apply H1.
-      * intro Hfv. inversion Hfv; subst.
-        ++ replace (S (S k)) with (swap01 (S (S k))) in H5 by auto.
-           apply fv_under_renaming in H5; try apply swap01_is_bijective.
-           apply H2. apply fv_cut_l.
-           apply fv_up_Sn2 in H5; auto; lia.
-        ++ apply H2. apply fv_cut_r.
-           replace (S (S k)) with (swap01 (S (S k))) in H5 by auto.
-           apply fv_under_renaming in H5; try apply swap01_is_bijective.
-           apply directed_cong_in_struct_cong in d.
-           assert ((S k) ∈ (cut Q R)) by (repeat free_var_econstructor; eauto).
-           apply ((proj1 free_vars_under_struct_cong) _ _ d) in H3. auto.
-      * intros [|[|]] ?; auto; exfalso; lia.
-      * intros [|[|]] ?; auto; exfalso; lia.
+      rewrite (proj1 down_k_down_Sj_lt_commute); auto; try lia.
+      intros [|[|]] ?; auto; exfalso; lia.
   + econstructor; try apply (H (S k)); try apply H0; intro Hfv; apply H1; free_var_econstructor; auto.
-  + econstructor; apply H; intro Hfv; apply H0; free_var_econstructor; auto. *)
-Admitted.
-
-(******************************************************************************)
-(* Transitivity is admissible                                                 *)
-(******************************************************************************)
-Lemma directed_cong_triangle :
-  (forall P1 P2, P1 ⇛ P2 -> forall P3, P1 ⇛ P3 -> P2 ⇛ P3) /\
-  (forall M1 M2, M1 !⇛ M2 -> forall M3, M1 !⇛ M3 -> M2 !⇛ M3) /\
-  (forall s1 s2, s1 $⇛ s2 -> forall s3, s1 $⇛ s3 -> s2 $⇛ s3).
-Proof.
-  (* apply directed_cong_ind; intros.
-  + inversion H1; subst.
-    - apply dc_cong_link; try apply H; try apply H0; auto.
-    - apply dc_link; try apply H; try apply H0; auto.
-  + inversion H1; subst.
-    - apply dc_link; try apply H; try apply H0; auto.
-    - apply dc_cong_link; try apply H; try apply H0; auto.
-  + admit.
-  (* + inversion H1; subst.
-    - apply dc_cong_cut; try apply H; try apply H0; eauto.
-    - assert ( P' ⇛ (cut P0 Q0) ) by apply (H _ H4).
-      (* show that if P ⇛ cut P0 Q0, then also P ⇛ cut Q0 P0 *)
-      (* and other direction as well since we haven't proven symmetry yet *)
-      assert ( P' ⇛ (cut Q0 P0) )
-        by admit.
-      eapply dc_cut_assoc_r_comm.
-      * apply H3.
-      * assumption.
-      * admit.
-      * auto.
-      * auto.
-      * auto.
-      * admit.
-    - admit.
-    - admit.
-    - admit.
-    - apply dc_cut_comm; try apply H; try apply H0; eauto. *)
-  + admit.
-  + admit.
-  + admit.
-  + admit.
-  + admit.
-  + inversion H1; subst; econstructor; eauto.
-  + inversion H; econstructor.
-  + inversion H0; econstructor; eauto. apply H. apply dc_cong_reflS.
-  + auto.
-  + inversion H0; econstructor; eauto. apply H. apply directed_cong_reflexive.
-  + inversion H0; econstructor; eauto. apply H. apply directed_cong_reflexive.
-  + inversion H1; econstructor; eauto; try apply H; try apply H0; apply directed_cong_reflexive.
-  + inversion H1; econstructor; eauto; try apply H; try apply H0; apply directed_cong_reflexive.
-  + inversion H0; econstructor; eauto. apply H. apply directed_cong_reflexive.
-  + inversion H; econstructor.
-  + inversion H0; econstructor; eauto. apply H. apply directed_cong_reflexive.
-  + auto. *)
-Admitted.
+  + econstructor; apply H; intro Hfv; apply H0; free_var_econstructor; auto.
+Qed.
 
 (******************************************************************************)
 (* Symmetry is admissible                                                     *)
 (******************************************************************************)
-(* Lemma directed_cong_cut_comm_common_reduct :
-  forall P1 P2 Q, (cut P1 P2) ⇛ Q -> (cut P2 P1) ⇛ Q.
-Proof.
-  intros.
-  generalize dependent P1.
-  generalize dependent P2.
-  induction Q; intros; try (now (inversion H)).
-  inversion H; subst.
-  + apply dc_cong_cut; auto.
-  + 
-    admit.
-  + admit.
-  + admit.
-  + admit.
-  + apply dc_cut_comm; auto.
-Admitted. *)
-
 Lemma directed_cong_symm :
   (forall P1 P2, P1 ⇛ P2 -> P2 ⇛ P1) /\
   (forall M1 M2, M1 !⇛ M2 -> M2 !⇛ M1) /\
   (forall s1 s2, s1 $⇛ s2 -> s2 $⇛ s1).
 Proof.
   apply directed_cong_ind; intros; try now (econstructor; eauto).
-  + assert ((down (rename_process P' swap01)) ⇛ (down (rename_process P swap01))).
-    {
-      apply directed_cong_invariant_under_downshifting.
-      + apply directed_cong_invariant_under_renaming; auto. apply swap01_is_bijective.
-      + apply nfv_01_swap. intro Hfv.
-        apply directed_cong_in_struct_cong in d0. apply c_comm in d0.
-        apply (proj1 free_vars_under_struct_cong) with (k := 1) in d0. apply n.
-        apply d0. auto.
-    }
-    eapply dc_cut_assoc_r1.
-    - apply H2.
-    - rewrite e1. apply nfv_10_swap. apply nfv_lift_n; lia.
-    - rewrite e. apply H3.
-    - assert (
-        (rename_process (up R') swap01) ⇛ (rename_process (up R) swap01)
-      ).
-      {
-        apply directed_cong_invariant_under_renaming; try apply swap01_is_bijective.
-        apply directed_cong_invariant_under_upshifting; auto.
-      }
-      rewrite e1. apply H4.
-    - autorewrite with up_down_rename_rewrites. reflexivity.
-      apply nfv_01_swap; auto.
-    - rewrite e0. autorewrite with up_down_rename_rewrites; auto.
-    - subst; autorewrite with up_down_rename_rewrites; auto.
-    - apply H.
-  + assert ((down (rename_process P' swap01)) ⇛ (down (rename_process P swap01))).
-    {
-      apply directed_cong_invariant_under_downshifting.
-      + apply directed_cong_invariant_under_renaming; auto. apply swap01_is_bijective.
-      + apply nfv_01_swap. intro Hfv.
-        apply directed_cong_in_struct_cong in d0. apply c_comm in d0.
-        apply (proj1 free_vars_under_struct_cong) with (k := 1) in d0. apply n.
-        apply d0. auto.
-    }
-    eapply dc_cut_assoc_r2.
-    - apply H2.
-    - rewrite e1. apply nfv_10_swap. apply nfv_lift_n; lia.
-    - rewrite e. apply H3.
-    - assert (
-        (rename_process (up R') swap01) ⇛ (rename_process (up R) swap01)
-      ).
-      {
-        apply directed_cong_invariant_under_renaming; try apply swap01_is_bijective.
-        apply directed_cong_invariant_under_upshifting; auto.
-      }
-      rewrite e1. apply H4.
-    - autorewrite with up_down_rename_rewrites. reflexivity.
-      apply nfv_01_swap. auto.
-    - rewrite e0. autorewrite with up_down_rename_rewrites; auto.
-    - subst; autorewrite with up_down_rename_rewrites; auto.
-    - auto.
-  + admit.
-  + admit.
-
-    (* assert ((rename_process Q1 swap01) ⇛ (rename_process Q swap01)).
+  + assert ((rename_process Q1 swap01) ⇛ (rename_process Q swap01)).
     { apply directed_cong_invariant_under_renaming; auto. apply swap01_is_bijective. }
     assert ((rename_process (up R1) swap01) ⇛ (rename_process (up R) swap01)).
     {
@@ -1504,7 +795,11 @@ Proof.
       (down (rename_process (rename_process (up R) swap01) swap01))
       by (autorewrite with up_down_rename_rewrites; eauto).
     subst.
-    eapply c_cut_assoc_r; eauto. apply nfv_10_swap. apply nfv_lift_n. lia.
+    eapply dc_cut_assoc_r; eauto. apply nfv_10_swap. apply nfv_lift_n. lia.
+    apply directed_cong_invariant_under_downshifting.
+    apply directed_cong_invariant_under_renaming; auto. apply swap01_is_bijective.
+    apply nfv_01_swap. intro Hfv. apply directed_cong_in_struct_cong in H.
+    apply ((proj1 free_vars_under_struct_cong) _ _ H) in Hfv; congruence.
   + assert ((rename_process (up P1) swap01) ⇛ (rename_process (up P) swap01)).
     {
       apply directed_cong_invariant_under_renaming.
@@ -1532,8 +827,8 @@ Proof.
       (rename_process (up (down (rename_process R swap01))) swap01)
       by (autorewrite with up_down_rename_rewrites; try eapply nfv_01_swap; eauto).
     subst.
-    eapply c_cut_assoc_l; eauto. apply nfv_10_swap. apply nfv_lift_n. lia. *)
-Admitted.
+    eapply dc_cut_assoc_l; eauto. apply nfv_10_swap. apply nfv_lift_n. lia.
+Qed.
 
 Corollary directed_cong_symmetric : symmetric _ directed_congruence.
 Proof. unfold symmetric; intros. apply (proj1 directed_cong_symm) in H. auto. Qed.
@@ -1648,4 +943,714 @@ Proof.
   + clear s. induction H; intros.
     - repeat econstructor; eauto.
     - eapply Relation_Operators.t1n_trans. { econstructor; eauto. } apply IHclos_trans_1n.
+Qed.
+
+(******************************************************************************)
+(* Directed congruence is invariant under substitution                        *)
+(******************************************************************************)
+Definition subst_dc_equiv (σ1 σ2 : substitution) : Prop :=
+  forall i, (σ1 i) !⇛ (σ2 i).
+
+Lemma subst_dc_equiv_refl :
+  (forall P, forall σ1 σ2, subst_dc_equiv σ1 σ2
+    -> (subst_process P σ1) ⇛ (subst_process P σ2)) /\
+  (forall M, forall σ1 σ2, subst_dc_equiv σ1 σ2
+    -> (subst_message M σ1) !⇛ (subst_message M σ2)) /\
+  (forall s, forall σ1 σ2, subst_dc_equiv σ1 σ2
+    -> (subst_statement s σ1) $⇛ (subst_statement s σ2)).
+Proof.
+  apply syntax_ind; intros; simpl;
+  assert (subst_dc_equiv (up_subst σ1) (up_subst σ2)) by
+    (intros [|]; simpl; try econstructor; apply directed_cong_invariant_under_upshifting; auto);
+  try (now (econstructor; try apply H; try apply H0; eauto)).
+  + apply (H n).
+  + econstructor. apply H. intros [|]; simpl; try econstructor;
+    apply directed_cong_invariant_under_upshifting; auto.
+Qed.
+
+(* r identity after k and for all i: ren (σ i) r = σ i *)
+(* show in a separate lemma: forall k, j < k -> j free and for all j >= k: r j = j,
+   then renaming idempotent OR:
+   forall i, r i ≠ i, i not free -> renaming idempotent
+   *)
+Fixpoint up_subst_n (n : nat) (σ : substitution) : substitution :=
+  match n with
+  | O    => σ
+  | S n' => up_subst (up_subst_n n' σ)
+  end.
+
+(* Properties about up_subst_n *)
+Lemma up_subst_n_lt :
+  forall n k σ, n < k -> up_subst_n k σ n = future n.
+Proof.
+  intros.
+  generalize dependent n.
+  induction k; intros.
+  + inversion H.
+  + simpl. destruct n; auto.
+    simpl. rewrite IHk; auto. lia.
+Qed.
+
+Lemma up_subst_n_ge :
+  forall n k σ, k <= n -> up_subst_n k σ n = lift_message (σ (n - k)) 0 k.
+Proof.
+  intros.
+  generalize dependent n.
+  induction k; intros.
+  + rewrite PeanoNat.Nat.sub_0_r; simpl.
+    rewrite (proj1 (proj2 shift_with_0_idempotent)). auto.
+  + simpl. assert (k <= n) by lia. destruct n; try (exfalso; lia).
+    simpl. rewrite IHk; try lia. unfold upM.
+    rewrite (proj1 (proj2 shift_additive)). replace (k + 1) with (S k) by lia.
+    auto.
+Qed.
+
+Lemma shift_shift_raise_bound :
+  (forall P n1 n2 k1 k2, n1 <= n2 -> n2 <= n1 + k1 ->
+    (lift_process (lift_process P n1 k1) n2 k2) =
+    (lift_process (lift_process P n1 k1) (n1 + k1) k2)) /\
+  (forall M n1 n2 k1 k2, n1 <= n2 -> n2 <= n1 + k1 ->
+    (lift_message (lift_message M n1 k1) n2 k2) =
+    (lift_message (lift_message M n1 k1) (n1 + k1) k2)) /\
+  (forall s n1 n2 k1 k2, n1 <= n2 -> n2 <= n1 + k1 ->
+    (lift_statement (lift_statement s n1 k1) n2 k2) =
+    (lift_statement (lift_statement s n1 k1) (n1 + k1) k2)).
+Proof.
+  apply syntax_ind; intros; simpl; try rewrite H; try rewrite H0; auto; try lia.
+  unfold relocate.
+  destruct (Nat.leb n1 n) eqn:E.
+  + apply PeanoNat.Nat.leb_le in E. assert (n2 <= k1 + n) by lia.
+    apply PeanoNat.Nat.leb_le in H1. rewrite H1.
+    assert (n1 <= k1 + n) by lia. assert (n1 + k1 <= k1 + n) by lia.
+    apply PeanoNat.Nat.leb_le in H3. rewrite H3. auto.
+  + apply PeanoNat.Nat.leb_nle in E.
+    assert (~ (n2 <= n)) by lia. apply PeanoNat.Nat.leb_nle in H1.
+    assert (~ (n1 + k1 <= n)) by lia. apply PeanoNat.Nat.leb_nle in H2.
+    rewrite H1. rewrite H2. auto.
+Qed.
+
+Lemma subst_up_lift_commute :
+  (forall P, forall σ k,
+    subst_process (lift_process P k 1) (up_subst_n (S k) σ)
+      = lift_process (subst_process P (up_subst_n k σ)) k 1)
+  /\
+  (forall M, forall σ k,
+    subst_message (lift_message M k 1) (up_subst_n (S k) σ)
+      = lift_message (subst_message M (up_subst_n k σ)) k 1)
+  /\
+  (forall s, forall σ k,
+    subst_statement (lift_statement s k 1) (up_subst_n (S k) σ)
+      = lift_statement (subst_statement s (up_subst_n k σ)) k 1).
+Proof.
+  apply syntax_ind; intros; simpl;
+  try replace (up_subst (up_subst_n k σ)) with (up_subst_n (S k) σ) by auto;
+  try replace (up_subst (up_subst_n (S k) σ)) with (up_subst_n (S (S k)) σ) by auto;
+  try now (try rewrite H; try rewrite H0; auto).
+  + simpl. unfold relocate.
+    destruct (Nat.leb k n) eqn:E.
+    - simpl. apply PeanoNat.Nat.leb_le in E. unfold upM.
+      rewrite up_subst_n_ge; auto.
+      rewrite ((proj1 (proj2 shift_shift_raise_bound)) _ 0 0 k 1); try lia. auto.
+    - apply PeanoNat.Nat.leb_nle in E.
+      assert (n < k) by lia.
+      assert (n < S k) by lia.
+      replace (up_subst (up_subst_n k σ)) with (up_subst_n (S k) σ) by auto.
+      assert (up_subst_n (S k) σ n = future n) by (apply up_subst_n_lt; auto).
+      rewrite H1.
+      assert (up_subst_n k σ n = future n) by (apply up_subst_n_lt; auto).
+      rewrite H2. simpl. unfold relocate. apply PeanoNat.Nat.leb_nle in E. rewrite E.
+      auto.
+  + replace (up_subst (up_subst_n (S (S k)) σ)) with (up_subst_n (S (S (S k))) σ) by auto.
+    rewrite H. auto.
+Qed.
+
+Lemma down_after_lift_Sk :
+  (forall P, forall n1 k,
+    down1_process (lift_process P n1 (S k)) (n1 + k) = lift_process P n1 k)
+  /\
+  (forall M, forall n1 k,
+    down1_message (lift_message M n1 (S k)) (n1 + k) = lift_message M n1 k)
+  /\
+  (forall s, forall n1 k,
+    down1_statement (lift_statement s n1 (S k)) (n1 + k) = lift_statement s n1 k).
+Proof.
+  apply syntax_ind; intros; simpl; try rewrite H; try rewrite H0; auto; try lia.
+  unfold relocate.
+  destruct (Nat.leb n1 n) eqn:E; simpl.
+  + apply PeanoNat.Nat.leb_le in E. assert (n1 + k < S (k + n)) by lia.
+    apply PeanoNat.Nat.ltb_lt in H. rewrite H; auto.
+  + apply PeanoNat.Nat.leb_nle in E. assert (~ (n1 + k <  n)) by lia.
+    apply PeanoNat.Nat.ltb_nlt in H. rewrite H; auto.
+Qed.
+
+Lemma subst_up_down_commute :
+  (forall P, forall σ k,
+    ~ (k ∈ P) ->
+    down1_process (subst_process P (up_subst_n (S k) σ)) k =
+    subst_process (down1_process P k) (up_subst_n k σ)) /\
+  (forall M, forall σ k,
+    ~ (occurs_free_message k M) ->
+    down1_message (subst_message M (up_subst_n (S k) σ)) k =
+    subst_message (down1_message M k) (up_subst_n k σ)) /\
+  (forall s, forall σ k,
+    ~ (occurs_free_statement k s) ->
+    down1_statement (subst_statement s (up_subst_n (S k) σ)) k =
+    subst_statement (down1_statement s k) (up_subst_n k σ)).
+Proof.
+  apply syntax_ind; intros; simpl;
+  try replace (up_subst (up_subst_n k σ)) with (up_subst_n (S k) σ) by auto;
+  try replace (up_subst (up_subst_n (S k) σ)) with (up_subst_n (S (S k)) σ) by auto;
+  try (now (try rewrite H; try rewrite H0; auto; intro Hfv; try apply H1; try apply H0; free_var_econstructor; eauto)).
+  + destruct (Nat.ltb k n) eqn:E.
+    - apply PeanoNat.Nat.ltb_lt in E.
+      assert (S k <= n) by lia.
+      assert (up_subst_n (S k) σ n = lift_message (σ (n - (S k))) 0 (S k))
+        by (apply up_subst_n_ge; auto).
+      rewrite H1. simpl.
+      assert (up_subst_n k σ (Nat.pred n) = lift_message (σ (Nat.pred n - k)) 0 k).
+      { rewrite up_subst_n_ge; auto. lia. }
+      rewrite  H2. simpl.
+      assert (n - S k = Nat.pred n - k) by lia.
+      rewrite H3. rewrite (proj1 (proj2 down_after_lift_Sk)). auto.
+    - apply PeanoNat.Nat.ltb_nlt in E.
+      assert (n < (S k)) by lia.
+      assert (up_subst_n (S k) σ n = future n) by (apply up_subst_n_lt; auto).
+      rewrite H1. simpl. apply PeanoNat.Nat.ltb_nlt in E. rewrite E.
+      apply PeanoNat.Nat.ltb_nlt in E.
+      assert (n <> k). { intro Heq. apply H. rewrite Heq; econstructor. }
+      assert (n < k) by lia.
+      assert (up_subst_n k σ n = future n) by (apply up_subst_n_lt; auto).
+      rewrite H4.
+      auto.
+  + replace (up_subst (up_subst_n (S (S k)) σ)) with (up_subst_n (S (S (S k))) σ) by auto.
+    rewrite H; auto. intro Hfv. apply H0. free_var_econstructor. auto.
+Qed.
+
+Lemma ren_subst_commute :
+  (forall P, forall r σ k,
+    bijective r -> (forall j, j >= k -> r j = j) ->
+    (forall j, j < k -> (σ j) = (future j)) ->
+    (forall j, j >= k -> (rename_message (σ j) r) = (σ j)) ->
+    subst_process (rename_process P r) σ
+      = rename_process (subst_process P σ) r)
+  /\
+  (forall M, forall r σ k,
+    bijective r -> (forall j, j >= k -> r j = j) ->
+    (forall j, j < k -> (σ j) = (future j)) ->
+    (forall j, j >= k -> (rename_message (σ j) r) = (σ j)) ->
+    subst_message (rename_message M r) σ
+      = rename_message (subst_message M σ) r)
+  /\
+  (forall s, forall r σ k,
+    bijective r -> (forall j, j >= k -> r j = j) ->
+    (forall j, j < k -> (σ j) = (future j)) ->
+    (forall j, j >= k -> (rename_message (σ j) r) = (σ j)) ->
+    subst_statement (rename_statement s r) σ
+      = rename_statement (subst_statement s σ) r).
+Proof.
+  apply syntax_ind; intros; simpl;
+  try now (try rewrite (H _ _ k); try rewrite (H0 _ _ k); auto).
+  + assert (
+      forall j : nat, j >= (S k) -> up_ren r j = j
+    ).
+    { intros [|] ?; auto; simpl. rewrite H2; auto; lia. }
+    assert (
+      forall j : nat, j < S k -> up_subst σ j = future j
+    ).
+    {
+      intros [|] ?; auto; simpl. rewrite H3; simpl; auto; lia.
+    }
+    assert (
+      forall j : nat, j >= S k -> rename_message (up_subst σ j) (up_ren r) = up_subst σ j
+    ).
+    {
+      intros [|] ?; auto; simpl.
+      unfold upM.
+      rewrite (proj1 (proj2 ren_up_up_ren_commute)); auto.
+      + rewrite H4; auto; lia.
+      + intros; exfalso; lia.
+    }
+    assert (
+      bijective (up_ren r)
+    ) by (apply shift_preserves_bijection; auto).
+    rewrite (H _ _ (S k)); try rewrite (H0 _ _ (S k)); auto.
+  + assert (
+      forall j : nat, j >= (S k) -> up_ren r j = j
+    ).
+    { intros [|] ?; auto; simpl. rewrite H2; auto; lia. }
+    assert (
+      forall j : nat, j < S k -> up_subst σ j = future j
+    ).
+    {
+      intros [|] ?; auto; simpl. rewrite H3; simpl; auto; lia.
+    }
+    assert (
+      forall j : nat, j >= S k -> rename_message (up_subst σ j) (up_ren r) = up_subst σ j
+    ).
+    {
+      intros [|] ?; auto; simpl.
+      unfold upM.
+      rewrite (proj1 (proj2 ren_up_up_ren_commute)); auto.
+      + rewrite H4; auto; lia.
+      + intros; exfalso; lia.
+    }
+    assert (
+      bijective (up_ren r)
+    ) by (apply shift_preserves_bijection; auto).
+    rewrite (H _ _ (S k)); try rewrite (H0 _ _ (k)); auto.
+  + destruct (Compare_dec.lt_dec n k).
+    - rewrite H1. rewrite H1; simpl. auto. auto.
+      destruct (Compare_dec.lt_dec (r n) k); auto.
+      apply Compare_dec.not_lt in n0.
+      rewrite H0 in n0; try lia.
+      assert ( (r (r n)) = (r n)). { rewrite H0; auto. }
+      assert (r n = n).
+      {
+        destruct H. assert (g (r (r n)) = g (r n)) by auto.
+        rewrite c in H. rewrite c in H. auto.
+      }
+      rewrite <- H4; auto.
+    - apply Compare_dec.not_lt in n0. rewrite H0; auto.
+      rewrite H2; auto.
+  + assert (
+      forall j : nat, j >= (S k) -> up_ren r j = j
+    ).
+    { intros [|] ?; auto; simpl. rewrite H1; auto; lia. }
+    assert (
+      forall j : nat, j < S k -> up_subst σ j = future j
+    ).
+    {
+      intros [|] ?; auto; simpl. rewrite H2; simpl; auto; lia.
+    }
+    assert (
+      forall j : nat, j >= S k -> rename_message (up_subst σ j) (up_ren r) = up_subst σ j
+    ).
+    {
+      intros [|] ?; auto; simpl.
+      unfold upM.
+      rewrite (proj1 (proj2 ren_up_up_ren_commute)); auto.
+      + rewrite H3; auto; lia.
+      + intros; exfalso; lia.
+    }
+    assert (
+      bijective (up_ren r)
+    ) by (apply shift_preserves_bijection; auto).
+    rewrite (H _ _ (S k)); try rewrite (H0 _ _ (S k)); auto.
+  + assert (
+      forall j : nat, j >= (S k) -> up_ren r j = j
+    ).
+    { intros [|] ?; auto; simpl. rewrite H1; auto; lia. }
+    assert (
+      forall j : nat, j < S k -> up_subst σ j = future j
+    ).
+    {
+      intros [|] ?; auto; simpl. rewrite H2; simpl; auto; lia.
+    }
+    assert (
+      forall j : nat, j >= S k -> rename_message (up_subst σ j) (up_ren r) = up_subst σ j
+    ).
+    {
+      intros [|] ?; auto; simpl.
+      unfold upM.
+      rewrite (proj1 (proj2 ren_up_up_ren_commute)); auto.
+      + rewrite H3; auto; lia.
+      + intros; exfalso; lia.
+    }
+    assert (
+      bijective (up_ren r)
+    ) by (apply shift_preserves_bijection; auto).
+    rewrite (H _ _ (S k)); try rewrite (H0 _ _ (S k)); auto.
+  + assert (
+      forall j : nat, j >= (S k) -> up_ren r j = j
+    ).
+    { intros [|] ?; auto; simpl. rewrite H2; auto; lia. }
+    assert (
+      forall j : nat, j < S k -> up_subst σ j = future j
+    ).
+    {
+      intros [|] ?; auto; simpl. rewrite H3; simpl; auto; lia.
+    }
+    assert (
+      forall j : nat, j >= S k -> rename_message (up_subst σ j) (up_ren r) = up_subst σ j
+    ).
+    {
+      intros [|] ?; auto; simpl.
+      unfold upM.
+      rewrite (proj1 (proj2 ren_up_up_ren_commute)); auto.
+      + rewrite H4; auto; lia.
+      + intros; exfalso; lia.
+    }
+    assert (
+      bijective (up_ren r)
+    ) by (apply shift_preserves_bijection; auto).
+    rewrite (H _ _ (S k)); try rewrite (H0 _ _ (S k)); auto.
+  + assert (
+      forall j : nat, j >= (S k) -> up_ren r j = j
+    ).
+    { intros [|] ?; auto; simpl. rewrite H2; auto; lia. }
+    assert (
+      forall j : nat, j < S k -> up_subst σ j = future j
+    ).
+    {
+      intros [|] ?; auto; simpl. rewrite H3; simpl; auto; lia.
+    }
+    assert (
+      forall j : nat, j >= S k -> rename_message (up_subst σ j) (up_ren r) = up_subst σ j
+    ).
+    {
+      intros [|] ?; auto; simpl.
+      unfold upM.
+      rewrite (proj1 (proj2 ren_up_up_ren_commute)); auto.
+      + rewrite H4; auto; lia.
+      + intros; exfalso; lia.
+    }
+    assert (
+      bijective (up_ren r)
+    ) by (apply shift_preserves_bijection; auto).
+    rewrite (H _ _ (S k)); try rewrite (H0 _ _ (S k)); auto.
+  + rewrite (H _ _ (S (S k))); auto.
+    - repeat apply shift_preserves_bijection; auto.
+    - intros [|[|]] ?; auto; simpl. rewrite H1; auto; lia.
+    - intros [|[|]] ?; auto; simpl. rewrite H2; simpl; auto; lia.
+    - intros [|[|]] ?; auto; simpl. unfold upM.
+      rewrite (proj1 (proj2 ren_up_up_ren_commute)); auto.
+      rewrite (proj1 (proj2 ren_up_up_ren_commute)); auto.
+      rewrite H3; auto. lia.
+      * intros; exfalso; lia.
+      * apply shift_preserves_bijection; auto.
+      * intros; exfalso; lia.
+Qed.
+
+Lemma fv_up_Sn2' :
+  (forall (p : process),
+    forall n k, k <= n -> (S n) ∈ (lift_process p k 1) -> n ∈ p)
+  /\
+  (forall (m : message),
+    forall n k, k <= n -> occurs_free_message (S n) (lift_message m k 1) -> occurs_free_message n m)
+  /\
+  (forall (s : statement),
+    forall n k, k <= n -> occurs_free_statement (S n) (lift_statement s k 1) -> occurs_free_statement n s).
+Proof.
+  apply syntax_ind; intros; simpl.
+  + simpl in H2; inversion H2; subst.
+    - apply fv_link_l. eapply (H n k); auto.
+    - apply fv_link_r. eapply (H0 n k); auto.
+  + simpl in H2; inversion H2; subst.
+    - apply fv_cut_l. eapply (H (S n) (S k)); auto. lia.
+    - apply fv_cut_r. eapply (H0 (S n) (S k)); auto. lia.
+  + simpl in H2; inversion H2; subst.
+    - apply fv_seq_l. eapply (H (S n) (S k)); auto. lia.
+    - apply fv_seq_r. eapply (H0 n k); auto.
+  + inversion H0.
+  + inversion H0; subst.
+    destruct (Nat.leb k n) eqn:E.
+    - unfold relocate in H3. rewrite E in H3. simpl in H3.
+      inversion H3. econstructor.
+    - unfold relocate in H3. rewrite E in H3.
+      rewrite H3 in H0. apply PeanoNat.Nat.leb_nle in E.
+      assert (n < n0) by lia. exfalso; lia.
+  + simpl in H1; inversion H1; subst. econstructor. eapply H; eauto.
+  + simpl in H1; inversion H1; subst. econstructor. eapply (H (S n) (S k)); eauto. lia.
+  + simpl in H1; inversion H1; subst. econstructor. eapply (H (S n) (S k)); eauto. lia.
+  + simpl in H2; inversion H2; subst.
+    - apply fv_choice_l. eapply (H (S n) (S k)); auto. lia.
+    - apply fv_choice_r. eapply (H0 (S n) (S k)); auto. lia.
+  + simpl in H2; inversion H2; subst.
+    - apply fv_send_l. eapply (H (S n) (S k)); auto. lia.
+    - apply fv_send_r. eapply (H0 (S n) (S k)); auto. lia.
+  + simpl in H1; inversion H1; subst; econstructor. eapply (H (S (S n)) (S (S k))); eauto; lia.
+  + inversion H0.
+  + inversion H1; subst. econstructor. eapply H; eauto.
+Qed.
+
+Lemma nfv_under_substitution :
+  (forall P σ i,
+    ~ (i ∈ P) ->
+    (forall n, n <> i -> ~ (occurs_free_message i (σ n)))
+    -> ~ (i ∈ (subst_process P σ))) /\
+  (forall M σ i,
+    ~ (occurs_free_message i M) ->
+    (forall n, n <> i -> ~ (occurs_free_message i (σ n)))
+    -> ~ (occurs_free_message i (subst_message M σ))) /\
+  (forall s σ i,
+    ~ (occurs_free_statement i s) ->
+    (forall n, n <> i -> ~ (occurs_free_message i (σ n)))
+    -> ~ (occurs_free_statement i (subst_statement s σ))).
+Proof.
+  apply syntax_ind; intros;
+  (* assert that up_subst σ also satisfies free variables condition *)
+  try assert ( Hfvup : forall n : nat, n <> S i -> ~ occurs_free_message (S i) (up_subst σ n))
+  by (
+    intros; intro Hfv2; destruct n; simpl in Hfv2; auto; [
+      inversion Hfv2
+    | apply fv_up_Sn2' in Hfv2;
+      try apply (proj1 (PeanoNat.Nat.succ_inj_wd_neg _ _)) in H3;
+      try apply (proj1 (PeanoNat.Nat.succ_inj_wd_neg _ _)) in H2; auto; try lia;
+      try apply (H2 n); try apply (H1 n); auto
+    ]
+  ).
+  + intro Hfv. inversion Hfv; subst.
+    - assert (~ (occurs_free_message i m)).
+      { intro Hfv1. apply H1; free_var_econstructor; eauto. }
+      apply (H σ i H3 H2); auto.
+    - assert (~ (occurs_free_message i m0)).
+      { intro Hfv1. apply H1; free_var_econstructor; eauto. }
+      apply (H0 σ i H3 H2); auto.
+  + intro Hfv; inversion Hfv; subst.
+    - eapply (H (up_subst σ) (S i)); auto.
+      intro Hfv1; apply H1; free_var_econstructor; auto.
+    - eapply (H0 (up_subst σ) (S i)); auto.
+      intro Hfv1; apply H1; free_var_econstructor; auto.
+  + intro Hfv; inversion Hfv; subst.
+    - eapply (H (up_subst σ) (S i)); auto.
+      intro Hfv1; apply H1; free_var_econstructor; auto.
+    - eapply (H0 σ i); auto.
+      intro Hfv1; apply H1; free_var_econstructor; auto.
+  + simpl. intros; auto.
+  + intro Hfv. destruct (PeanoNat.Nat.eq_dec n i).
+    - subst. apply H. free_var_econstructor.
+    - apply (H0 n n0). simpl in Hfv. auto.
+  + intro Hfv; inversion Hfv; subst.
+    eapply (H σ i); auto. intro Hfv1; apply H0; free_var_econstructor; auto.
+  + intro Hfv; inversion Hfv; subst.
+    eapply (H (up_subst σ) (S i)); auto. intro Hfv1; apply H0; free_var_econstructor; auto.
+  + intro Hfv; inversion Hfv; subst.
+    eapply (H (up_subst σ) (S i)); auto. intro Hfv1; apply H0; free_var_econstructor; auto.
+  + intro Hfv; inversion Hfv; subst.
+    - eapply (H (up_subst σ) (S i)); auto.
+      intro Hfv1; apply H1; free_var_econstructor; auto.
+    - eapply (H0 (up_subst σ) (S i)); auto.
+      intro Hfv1; apply H1; free_var_econstructor; auto.
+  + intro Hfv; inversion Hfv; subst.
+    - eapply (H (up_subst σ) (S i)); auto.
+      intro Hfv1; apply H1; free_var_econstructor; auto.
+    - eapply (H0 (up_subst σ) (S i)); auto.
+      intro Hfv1; apply H1; free_var_econstructor; auto.
+  + intro Hfv; inversion Hfv; subst.
+    eapply (H (up_subst (up_subst σ)) (S (S i))); auto.
+    - intros Hfv1; apply H0. free_var_econstructor. auto.
+    - intros; intro Hfv2; destruct n; simpl in Hfv2; auto; [
+        inversion Hfv2
+      | apply fv_up_Sn2' in Hfv2;
+        try apply (proj1 (PeanoNat.Nat.succ_inj_wd_neg _ _)) in H3;
+        try apply (proj1 (PeanoNat.Nat.succ_inj_wd_neg _ _)) in H2; auto; try lia;
+        try apply (Hfvup n); auto
+      ].
+  + simpl. intros; auto.
+  + intro Hfv; inversion Hfv; subst.
+    eapply (H σ i); auto. intro Hfv1; apply H0; free_var_econstructor; auto.
+Qed.
+
+Lemma renaming_idempotent_free_vars :
+  (forall P r,
+    (forall n, n ∈ P -> r n = n) ->
+    (rename_process P r) = P) /\
+  (forall M r,
+    (forall n, occurs_free_message n M -> r n = n) ->
+    (rename_message M r) = M) /\
+  (forall s r,
+    (forall n, occurs_free_statement n s -> r n = n) ->
+    (rename_statement s r) = s).
+Proof.
+  apply syntax_ind; intros; simpl;
+  try rewrite H; try rewrite H0; auto;
+  try (intros; apply H1; free_var_econstructor; auto);
+  try (intros; apply H0; free_var_econstructor; auto);
+  try (intros; destruct n; simpl; auto; rewrite H1; auto; free_var_econstructor; auto);
+  try (intros; destruct n; simpl; auto; rewrite H0; auto; free_var_econstructor; auto).
+  + econstructor.
+  + intros. destruct n as [|[|]]; auto; simpl. rewrite H0; auto.
+    free_var_econstructor; auto.
+Qed.
+
+Lemma directed_cong_invariant_under_substitution :
+  (forall P Q, P ⇛ Q -> forall σ1 σ2, subst_dc_equiv σ1 σ2
+    -> (subst_process P σ1) ⇛ (subst_process Q σ2)) /\
+  (forall M N, M !⇛ N -> forall σ1 σ2, subst_dc_equiv σ1 σ2
+    -> (subst_message M σ1) !⇛ (subst_message N σ2)) /\
+  (forall s t, s $⇛ t -> forall σ1 σ2, subst_dc_equiv σ1 σ2
+    -> (subst_statement s σ1) $⇛ (subst_statement t σ2)).
+Proof.
+  apply directed_cong_ind; intros; simpl;
+  assert (subst_dc_equiv (up_subst σ1) (up_subst σ2)) by
+    (intros [|]; simpl; try econstructor; apply directed_cong_invariant_under_upshifting; auto);
+  try (now (econstructor; try apply H; try apply H0; auto)).
+  + assert (subst_dc_equiv (up_subst (up_subst σ1)) (up_subst (up_subst σ2)))
+      by (intros [|]; simpl; try econstructor; apply directed_cong_invariant_under_upshifting; auto).
+    eapply dc_cut_assoc_l.
+    - apply nfv_under_substitution; intros; try congruence.
+      intro Hfv. destruct n0 as [|[|]]; try (exfalso; lia); simpl in Hfv; auto.
+      * inversion Hfv.
+      * unfold upM in Hfv.
+        rewrite (proj1 (proj2 shift_additive) _ 0 1 1) in Hfv; simpl in Hfv.
+        apply nfv_lift_n in Hfv. auto. lia.
+    - apply H; eauto.
+    - apply H0; eauto.
+    - apply H1; eauto.
+    - rewrite e.
+      assert (
+        rename_process (subst_process P1 (up_subst (up_subst σ2))) swap01 =
+        subst_process (rename_process P1 swap01) (up_subst (up_subst σ2))
+      ).
+      {
+        rewrite ((proj1 ren_subst_commute) _ _ _ 2); auto.
+        * apply swap01_is_bijective.
+        * intros [|[|]] ?; auto; exfalso; lia.
+        * intros [|[|]] ?; auto; exfalso; lia.
+        * intros. destruct j as [|[|]]; try (exfalso; lia); simpl.
+          apply renaming_idempotent_free_vars. intros [|[|]].
+          - simpl. unfold upM. rewrite (proj1 (proj2 shift_additive)); simpl.
+            intros.
+            assert (~ (occurs_free_message 0 (lift_message (σ2 n0) 0 2))).
+            { apply nfv_lift_n; lia. }
+            congruence.
+          - simpl. unfold upM. rewrite (proj1 (proj2 shift_additive)); simpl.
+            intros.
+            assert (~ (occurs_free_message 1 (lift_message (σ2 n0) 0 2))).
+            { apply nfv_lift_n; lia. }
+            congruence.
+          - auto.
+      }
+      rewrite H5.
+      unfold down. replace (up_subst σ2) with (up_subst_n 0 (up_subst σ2)) by auto.
+      replace (up_subst (up_subst_n 0 (up_subst σ2))) with (up_subst_n 1 (up_subst σ2)) by auto.
+      rewrite (proj1 subst_up_down_commute); auto.
+      apply nfv_01_swap. intro Hfv. apply directed_cong_in_struct_cong in d.
+      apply c_comm in d. apply ((proj1 free_vars_under_struct_cong) _ _ d) in Hfv. congruence.
+    - rewrite e0.
+      rewrite ((proj1 ren_subst_commute) _ _ _ 2); auto.
+      * apply swap01_is_bijective.
+      * intros [|[|]] ?; auto; exfalso; lia.
+      * intros [|[|]] ?; auto; exfalso; lia.
+      * intros. destruct j as [|[|]]; try (exfalso; lia); simpl.
+        apply renaming_idempotent_free_vars. intros [|[|]].
+        ** simpl. unfold upM. rewrite (proj1 (proj2 shift_additive)); simpl.
+           intros.
+           assert (~ (occurs_free_message 0 (lift_message (σ2 n0) 0 2))).
+           { apply nfv_lift_n; lia. }
+           congruence.
+        ** simpl. unfold upM. rewrite (proj1 (proj2 shift_additive)); simpl.
+           intros.
+           assert (~ (occurs_free_message 1 (lift_message (σ2 n0) 0 2))).
+           { apply nfv_lift_n; lia. }
+           congruence.
+        ** auto.
+    - rewrite e1.
+      assert (
+        subst_process (rename_process (up R1) swap01) (up_subst (up_subst σ2)) =
+        rename_process (subst_process (up R1) (up_subst (up_subst σ2))) swap01
+      ).
+      {
+        rewrite ((proj1 ren_subst_commute) _ _ _ 2); auto.
+        * apply swap01_is_bijective.
+        * intros [|[|]] ?; auto; exfalso; lia.
+        * intros [|[|]] ?; auto; exfalso; lia.
+        * intros. destruct j as [|[|]]; try (exfalso; lia); simpl.
+          apply renaming_idempotent_free_vars. intros [|[|]].
+          - simpl. unfold upM. rewrite (proj1 (proj2 shift_additive)); simpl.
+            intros.
+            assert (~ (occurs_free_message 0 (lift_message (σ2 n0) 0 2))).
+            { apply nfv_lift_n; lia. }
+            congruence.
+          - simpl. unfold upM. rewrite (proj1 (proj2 shift_additive)); simpl.
+            intros.
+            assert (~ (occurs_free_message 1 (lift_message (σ2 n0) 0 2))).
+            { apply nfv_lift_n; lia. }
+            congruence.
+          - auto.
+      }
+      rewrite H5. unfold up.
+      replace (up_subst σ2) with (up_subst_n 1 σ2) by auto.
+      rewrite (proj1 subst_up_lift_commute); auto.
+  + assert (subst_dc_equiv (up_subst (up_subst σ1)) (up_subst (up_subst σ2)))
+      by (intros [|]; simpl; try econstructor; apply directed_cong_invariant_under_upshifting; auto).
+    eapply dc_cut_assoc_r.
+    - apply nfv_under_substitution; intros; try congruence.
+      intro Hfv. destruct n0 as [|[|]]; try (exfalso; lia); simpl in Hfv; auto.
+      * inversion Hfv.
+      * unfold upM in Hfv.
+        rewrite (proj1 (proj2 shift_additive) _ 0 1 1) in Hfv; simpl in Hfv.
+        apply nfv_lift_n in Hfv. auto. lia.
+    - apply H; eauto.
+    - apply H0; eauto.
+    - apply H1; eauto.
+    - rewrite e.
+      assert (
+        subst_process (rename_process (up P1) swap01) (up_subst (up_subst σ2)) =
+        rename_process (subst_process (up P1) (up_subst (up_subst σ2))) swap01
+      ).
+      {
+        rewrite ((proj1 ren_subst_commute) _ _ _ 2); auto.
+        * apply swap01_is_bijective.
+        * intros [|[|]] ?; auto; exfalso; lia.
+        * intros [|[|]] ?; auto; exfalso; lia.
+        * intros. destruct j as [|[|]]; try (exfalso; lia); simpl.
+          apply renaming_idempotent_free_vars. intros [|[|]].
+          - simpl. unfold upM. rewrite (proj1 (proj2 shift_additive)); simpl.
+            intros.
+            assert (~ (occurs_free_message 0 (lift_message (σ2 n0) 0 2))).
+            { apply nfv_lift_n; lia. }
+            congruence.
+          - simpl. unfold upM. rewrite (proj1 (proj2 shift_additive)); simpl.
+            intros.
+            assert (~ (occurs_free_message 1 (lift_message (σ2 n0) 0 2))).
+            { apply nfv_lift_n; lia. }
+            congruence.
+          - auto.
+      }
+      rewrite H5. unfold up.
+      replace (up_subst σ2) with (up_subst_n 1 σ2) by auto.
+      rewrite (proj1 subst_up_lift_commute); auto.
+    - rewrite e0.
+      rewrite ((proj1 ren_subst_commute) _ _ _ 2); auto.
+      * apply swap01_is_bijective.
+      * intros [|[|]] ?; auto; exfalso; lia.
+      * intros [|[|]] ?; auto; exfalso; lia.
+      * intros. destruct j as [|[|]]; try (exfalso; lia); simpl.
+        apply renaming_idempotent_free_vars. intros [|[|]].
+        ** simpl. unfold upM. rewrite (proj1 (proj2 shift_additive)); simpl.
+           intros.
+           assert (~ (occurs_free_message 0 (lift_message (σ2 n0) 0 2))).
+           { apply nfv_lift_n; lia. }
+           congruence.
+        ** simpl. unfold upM. rewrite (proj1 (proj2 shift_additive)); simpl.
+           intros.
+           assert (~ (occurs_free_message 1 (lift_message (σ2 n0) 0 2))).
+           { apply nfv_lift_n; lia. }
+           congruence.
+        ** auto.
+    - rewrite e1.
+      assert (
+        rename_process (subst_process R1 (up_subst (up_subst σ2))) swap01 =
+        subst_process (rename_process R1 swap01) (up_subst (up_subst σ2))
+      ).
+      {
+        rewrite ((proj1 ren_subst_commute) _ _ _ 2); auto.
+        * apply swap01_is_bijective.
+        * intros [|[|]] ?; auto; exfalso; lia.
+        * intros [|[|]] ?; auto; exfalso; lia.
+        * intros. destruct j as [|[|]]; try (exfalso; lia); simpl.
+          apply renaming_idempotent_free_vars. intros [|[|]].
+          - simpl. unfold upM. rewrite (proj1 (proj2 shift_additive)); simpl.
+            intros.
+            assert (~ (occurs_free_message 0 (lift_message (σ2 n0) 0 2))).
+            { apply nfv_lift_n; lia. }
+            congruence.
+          - simpl. unfold upM. rewrite (proj1 (proj2 shift_additive)); simpl.
+            intros.
+            assert (~ (occurs_free_message 1 (lift_message (σ2 n0) 0 2))).
+            { apply nfv_lift_n; lia. }
+            congruence.
+          - auto.
+      }
+      rewrite H5.
+      unfold down. replace (up_subst σ2) with (up_subst_n 0 (up_subst σ2)) by auto.
+      replace (up_subst (up_subst_n 0 (up_subst σ2))) with (up_subst_n 1 (up_subst σ2)) by auto.
+      rewrite (proj1 subst_up_down_commute); auto.
+      apply nfv_01_swap. intro Hfv. apply directed_cong_in_struct_cong in d1.
+      apply c_comm in d1. apply ((proj1 free_vars_under_struct_cong) _ _ d1) in Hfv. congruence.
+  + apply subst_dc_equiv_refl; auto.
+  + econstructor. apply H. intros [|]; simpl; try econstructor;
+    apply directed_cong_invariant_under_upshifting; auto.
+  + apply subst_dc_equiv_refl; auto.
 Qed.
