formalization/ParallelReduction.v
@@ -11,112 +11,33 @@ From Stdlib Require Import Relations.Relation_Operators.
 From Stdlib Require Import Relations.Operators_Properties.
 From Stdlib Require Import Relation_Definitions.
 
-(* Definition link_future (P : process) (x : nat) (M : message) : Prop :=
-  P = (link (future x) M) \/ P = (link M (future x)). *)
-
 (* ⊵ trianglerighteq *)
-(* Reserved Notation "P ⊵ Q" (no associativity, at level 61).
-
-Inductive par_reduces : process -> process -> Prop :=
-  (* embed ⇛ into ⊵ *)
-  | rp_directed_cong : forall P Q, P ⇛ Q -> P ⊵ Q
-
-  (* duplicate β-redexes up to symmetry of links *)
-  | rp_tensor_par_1 : forall P P' Q Q' R R' P'',
-      P ⇛ P' -> Q ⇛ Q' -> R ⇛ R' -> P'' = rename_process (up P') swap01 ->
-      link (prefix (send P Q)) (prefix (receive R)) ⊵ (cut (cut R' P'')) Q'
-  | rp_tensor_par_2 : forall P P' Q Q' R R' P'',
-      P ⇛ P' -> Q ⇛ Q' -> R ⇛ R' -> P'' = rename_process (up P') swap01 ->
-      link (prefix (receive R)) (prefix (send P Q)) ⊵ (cut (cut R' P'')) Q'
-  | rp_plus_with_l1 : forall P P' Q Q' R R',
-      P ⇛ P' -> Q ⇛ Q' -> R ⇛ R' ->
-      link (prefix (choose_left P)) (prefix (offer_choice Q R)) ⊵ cut P' Q'
-  | rp_plus_with_l2 : forall P P' Q Q' R R',
-      P ⇛ P' -> Q ⇛ Q' -> R ⇛ R' ->
-      link (prefix (offer_choice Q R)) (prefix (choose_left P)) ⊵ cut P' Q'
-  | rp_plus_with_r1 : forall (P P' Q R R' : process),
-      P ⇛ P' -> R ⇛ R' ->
-      link (prefix (choose_right P)) (prefix (offer_choice Q R)) ⊵ cut P' R'
-  | rp_plus_with_r2 : forall (P P' Q R R' : process),
-      P ⇛ P' -> R ⇛ R' ->
-      link (prefix (offer_choice Q R)) (prefix (choose_right P)) ⊵ cut P' R'
-  | rp_one_bot1 : forall P P', P ⇛ P' -> link (prefix close) (prefix (wait P)) ⊵ P'
-  | rp_one_bot2 : forall P P', P ⇛ P' -> link (prefix (wait P)) (prefix close) ⊵ P'
-
-  (* duplicate AxCut up to commutation of cuts (and links) *)
-  | rp_ax_cut1 : forall Q M M' P P',
-      P ⇛ P' -> M !⇛ M' -> link_future Q 0 M ->
-      cut Q P ⊵ subst_process P' ((downM M') ⋅ id_subst)
-  | rp_ax_cut2 : forall Q M M' P P',
-      P ⇛ P' -> M !⇛ M' -> link_future Q 0 M ->
-      cut P Q ⊵ subst_process P' ((downM M') ⋅ id_subst)
-
-  (* duplicate AxCut up to association of cuts (and symmetry links) *)
-  | rp_ax_cut_assoc_1 : forall P P' P'' M M' M'' R R' R'' Q,
-      link_future Q 1 M -> P ⊵ P' -> M !⇛ M' -> R ⊵ R' ->
-      P'' = rename_process (up P') swap01 ->
-      M'' = rename_message M' swap01 ->
-      R'' = down (rename_process R' swap01) ->
-      cut P (cut Q R) ⊵ cut (subst_process P'' ((downM M'' ⋅ id_subst))) R''
-  | rp_ax_cut_assoc_2 : forall P P' P'' M M' M'' R R' R'' Q,
-      link_future Q 1 M -> P ⊵ P' -> M !⇛ M' -> R ⊵ R' ->
-      P'' = rename_process (up P') swap01 ->
-      M'' = rename_message M' swap01 ->
-      R'' = down (rename_process R' swap01) ->
-      cut P (cut R Q) ⊵ cut (subst_process P'' ((downM M'' ⋅ id_subst))) R''
-  | rp_ax_cut_assoc_3 : forall P P' P'' M M' M'' R R' R'' Q,
-      link_future Q 1 M -> P ⊵ P' -> M !⇛ M' -> R ⊵ R' ->
-      P'' = rename_process (up P') swap01 ->
-      M'' = rename_message M' swap01 ->
-      R'' = down (rename_process R' swap01) ->
-      cut (cut Q R) P ⊵ cut (subst_process P'' ((downM M'' ⋅ id_subst))) R''
-  | rp_ax_cut_assoc_4 : forall P P' P'' M M' M'' R R' R'' Q,
-      link_future Q 1 M -> P ⊵ P' -> M !⇛ M' -> R ⊵ R' ->
-      P'' = rename_process (up P') swap01 ->
-      M'' = rename_message M' swap01 ->
-      R'' = down (rename_process R' swap01) ->
-      cut (cut R Q) P ⊵ cut (subst_process P'' ((downM M'' ⋅ id_subst))) R''
-
-  (* seq *)
-  | rp_seq : forall P P' s s', P ⇛ P' -> s $⇛ s' ->
-      seq P s ⊵ subst_process P' ((prefix s') ⋅ id_subst)
-
-  (* congruences *)
-  | rp_cong_cut : forall P P' Q Q', P ⊵ P' -> Q ⊵ Q' -> cut P Q ⊵ cut P' Q'
-  | rp_cong_seq : forall P P' s s', P ⊵ P' -> s $⇛ s' -> seq P s ⊵ seq P' s'
-where
-  "P ⊵ Q" := (par_reduces P Q). *)
-
 Reserved Notation "P ⊵ Q" (no associativity, at level 61).
 
-Inductive par_reduces : process -> process -> Prop :=
-  (* embed ⇛ into ⊵ *)
-  | rp_directed_cong : forall P Q, P ⇛ Q -> P ⊵ Q
+Inductive equiv_reduces : process -> process -> Prop :=
+  (* make ⊵ reflexive *)
+  | rp_refl : forall P, P ⊵ P
 
   (* duplicate β-redexes up to symmetry of links *)
-  | rp_tensor_par_1 : forall P P' Q Q' R R' P'',
-      P ⇛ P' -> Q ⇛ Q' -> R ⇛ R' -> P'' = rename_process (up P') swap01 ->
-      link (prefix (send P Q)) (prefix (receive R)) ⊵ (cut (cut R' P'')) Q'
-  | rp_tensor_par_2 : forall P P' Q Q' R R' P'',
-      P ⇛ P' -> Q ⇛ Q' -> R ⇛ R' -> P'' = rename_process (up P') swap01 ->
-      link (prefix (receive R)) (prefix (send P Q)) ⊵ (cut (cut R' P'')) Q'
-  | rp_plus_with_l1 : forall P P' Q Q' R R',
-      P ⇛ P' -> Q ⇛ Q' -> R ⇛ R' ->
-      link (prefix (choose_left P)) (prefix (offer_choice Q R)) ⊵ cut P' Q'
-  | rp_plus_with_l2 : forall P P' Q Q' R R',
-      P ⇛ P' -> Q ⇛ Q' -> R ⇛ R' ->
-      link (prefix (offer_choice Q R)) (prefix (choose_left P)) ⊵ cut P' Q'
-  | rp_plus_with_r1 : forall (P P' Q R R' : process),
-      P ⇛ P' -> R ⇛ R' ->
-      link (prefix (choose_right P)) (prefix (offer_choice Q R)) ⊵ cut P' R'
-  | rp_plus_with_r2 : forall (P P' Q R R' : process),
-      P ⇛ P' -> R ⇛ R' ->
-      link (prefix (offer_choice Q R)) (prefix (choose_right P)) ⊵ cut P' R'
-  | rp_one_bot1 : forall P P', P ⇛ P' -> link (prefix close) (prefix (wait P)) ⊵ P'
-  | rp_one_bot2 : forall P P', P ⇛ P' -> link (prefix (wait P)) (prefix close) ⊵ P'
+  | rp_tensor_par_1 : forall P P' Q R,
+      P' = rename_process (up P) swap01 ->
+      link (prefix (send P Q)) (prefix (receive R)) ⊵ (cut (cut R P')) Q
+  | rp_tensor_par_2 : forall P P' Q R,
+      P' = rename_process (up P) swap01 ->
+      link (prefix (receive R)) (prefix (send P Q)) ⊵ (cut (cut R P')) Q
+  | rp_plus_with_l1 : forall P Q R,
+      link (prefix (choose_left P)) (prefix (offer_choice Q R)) ⊵ cut P Q
+  | rp_plus_with_l2 : forall P Q R,
+      link (prefix (offer_choice Q R)) (prefix (choose_left P)) ⊵ cut P Q
+  | rp_plus_with_r1 : forall P Q R,
+      link (prefix (choose_right P)) (prefix (offer_choice Q R)) ⊵ cut P R
+  | rp_plus_with_r2 : forall P Q R,
+      link (prefix (offer_choice Q R)) (prefix (choose_right P)) ⊵ cut P R
+  | rp_one_bot1 : forall P, link (prefix close) (prefix (wait P)) ⊵ P
+  | rp_one_bot2 : forall P, link (prefix (wait P)) (prefix close) ⊵ P
 
   (* duplicate AxCut up to commutation and association of cuts *)
-  | rp_ax_cut : forall M M' P P',
+  (* | rp_ax_cut : forall M M' P P',
       P ⇛ P' -> M !⇛ M' -> (* !!!!!!!! this should be P ⊵ P' ??? or can we get away with ⇛ (I think this is the way, less effort ;) 
                                 not sure though if this work because of rp_cong_cut (but since redexes do not overlap, i.e.
                                 we dont really need a simultaneous reduction, this should be fine and if there are multiple
@@ -138,32 +59,39 @@ Inductive par_reduces : process -> process -> Prop :=
       P'' = down (rename_process P' swap01) ->
       M'' = rename_message M' swap01 ->
       R'' = rename_process (up R') swap01 ->
-      cut (cut P (link (future 1) M)) R ⊵ cut P'' (subst_process R'' ((downM M'' ⋅ id_subst)))
+      cut (cut P (link (future 1) M)) R ⊵ cut P'' (subst_process R'' ((downM M'' ⋅ id_subst))) *)
 
   (* seq *)
-  | rp_seq : forall P P' s s', P ⇛ P' -> s $⇛ s' ->
-      seq P s ⊵ subst_process P' ((prefix s') ⋅ id_subst)
+  | rp_seq : forall P s, seq P s ⊵ subst_process P ((prefix s) ⋅ id_subst)
 
   (* congruences *)
-  | rp_cong_cut : forall P P' Q Q', P ⊵ P' -> Q ⊵ Q' -> cut P Q ⊵ cut P' Q'
-  | rp_cong_seq : forall P P' s s', P ⊵ P' -> s $⇛ s' -> seq P s ⊵ seq P' s'
+  | rp_cong_cut_l : forall P P' Q, P ⊵ P' -> cut P Q ⊵ cut P' Q
+  | rp_cong_cut_r : forall P Q Q', Q ⊵ Q' -> cut P Q ⊵ cut P Q'
+  | rp_cong_seq : forall P P' s, P ⊵ P' -> seq P s ⊵ seq P' s
 where
-  "P ⊵ Q" := (par_reduces P Q).
+  "P ⊵ Q" := (equiv_reduces P Q).
 
-Lemma clos_trans_1n_directed_cong_in_clos_trans_1n_par_reduces :
-  forall P Q, (clos_trans_1n _ directed_congruence) P Q -> (clos_trans_1n _ par_reduces) P Q.
+Definition par_reduction := (union _ equiv_reduces structural_congruence).
+
+(* twoheadrightarrow *)
+Notation "P '↠' Q" := (par_reduction P Q) (no associativity, at level 61).
+
+(* ⇛* ⊂ ↠* *)
+Lemma clos_trans_1n_directed_cong_in_clos_trans_1n_par_reduction :
+  forall P Q, (clos_trans_1n _ directed_congruence) P Q -> (clos_trans_1n _ par_reduction) P Q.
 Proof.
   intros. induction H.
-  + econstructor. econstructor. assumption.
+  + econstructor. right. econstructor. apply c_comm. apply directed_cong_in_struct_cong. auto.
   + eapply Relation_Operators.t1n_trans.
-    - econstructor; eauto.
+    - right. apply directed_cong_in_struct_cong. eassumption.
     - auto.
 Qed.
 
-Lemma single_step_struct_cong_in_clos_trans_par_red :
-  forall P Q, (union _ reduces structural_congruence) P Q -> (clos_trans _ par_reduces) P Q.
+(* (▷ ∪ ≡) ⊂ ↠* *)
+Lemma single_step_struct_cong_in_clos_trans_par_reduction :
+  forall P Q, (union _ reduces structural_congruence) P Q -> (clos_trans _ par_reduction) P Q.
 Proof.
-  intros. destruct H.
+  (* intros. destruct H.
   + induction H.
     - econstructor. eapply rp_tensor_par_1; eauto; apply c_refl.
     - econstructor. eapply rp_plus_with_l1; eauto; apply c_refl.
@@ -186,14 +114,15 @@ Proof.
       eapply t_trans; eauto. eapply t_trans; eauto.
   + apply (proj1 struct_cong_in_trans_directed_cong) in H.
     apply clos_trans_t1n_iff.
-    apply clos_trans_1n_directed_cong_in_clos_trans_1n_par_reduces. auto.
-Qed.
+    apply clos_trans_1n_directed_cong_in_clos_trans_1n_par_reduces. auto. *)
+Admitted.
 
+(* ▶ ⊂ ↠* *)
 Lemma multi_step_red_in_clos_trans_par_red :
-  forall P Q, P ▶ Q -> (clos_trans _ par_reduces) P Q.
+  forall P Q, P ▶ Q -> (clos_trans _ par_reduction) P Q.
 Proof.
   intros. induction H.
-  + apply single_step_struct_cong_in_clos_trans_par_red in H. auto.
+  + apply single_step_struct_cong_in_clos_trans_par_reduction in H. auto.
   + eapply Relation_Operators.t_trans; eauto.
 Qed.
 
@@ -204,8 +133,36 @@ Ltac directed_cong_to_struct_cong :=
   | [ H : _ $⇛ _ |- _ ] => apply directed_cong_in_struct_cong in H
   end.
 
-Lemma par_reduces_in_union_single_step_red_struct_cong :
-  forall P Q, P ⊵ Q -> clos_trans _ (union _ reduces structural_congruence) P Q.
+(* ⊵ ⊂ (⊳ ∪ ≡) *)
+Lemma equiv_reduces_in_reduces_or_struct_cong :
+  forall P Q, P ⊵ Q -> (union _ reduces structural_congruence) P Q.
+Proof.
+  intros. induction H;
+  try (now (left; econstructor; eauto));
+  try (now (left; eapply r_struct; [ apply c_link | econstructor; eauto | apply c_refl ])).
+  + right. apply c_refl.
+  + destruct IHequiv_reduces.
+    - left. apply r_cong_cut. auto.
+    - right. apply c_cong_cut; auto. apply c_refl.
+  + destruct IHequiv_reduces.
+    - left. eapply r_struct. apply c_cut_comm. apply r_cong_cut. eauto. apply c_cut_comm.
+    - right. apply c_cong_cut; auto. apply c_refl.
+  + destruct IHequiv_reduces.
+    - left. apply r_cong_seq; auto.
+    - right. apply c_cong_seq; auto. apply struct_cong_reflS.
+Qed.
+
+(* ↠ ∪ (⊳ ∪ ≡) *)
+Lemma par_reduction_in_reduces_or_struct_cong :
+  forall P Q, P ↠ Q -> (union _ reduces structural_congruence) P Q.
+Proof.
+  intros. destruct H.
+  - apply equiv_reduces_in_reduces_or_struct_cong; auto.
+  - right; auto.
+Qed.
+
+(* Lemma par_reduces_in_union_single_step_red_struct_cong :
+  forall P Q, P ↠ Q -> clos_trans _ (union _ reduces structural_congruence) P Q.
 Proof.
   intros. induction H.
   + econstructor. apply directed_cong_in_struct_cong in H. right. auto.
@@ -401,26 +358,21 @@ Proof.
         destruct ((proj2 (proj2 struct_cong_d_refl)) s').
         eapply (proj2 (proj2 struct_cong_from_struct_cong_d)); eauto.
     - eapply t_trans; eauto.
-Qed.
+Admitted. *)
 
+(* ↠* ∪ ▶ *)
 Corollary clos_trans_par_red_in_multi_step_red :
-  forall P Q, clos_trans process par_reduces P Q -> P ▶ Q.
+  forall P Q, clos_trans process par_reduction P Q -> P ▶ Q.
 Proof.
   intros. induction H.
-  + apply par_reduces_in_union_single_step_red_struct_cong in H; auto.
+  + apply t_step. apply par_reduction_in_reduces_or_struct_cong. auto.
   + eapply t_trans; eauto.
 Qed.
 
 Corollary par_reds_clos_trans_multi_step_red_coincide :
-  forall P Q, (clos_trans _ par_reduces) P Q <-> P ▶ Q.
+  forall P Q, (clos_trans _ par_reduction) P Q <-> P ▶ Q.
 Proof.
   intros; split.
   + apply clos_trans_par_red_in_multi_step_red.
   + apply multi_step_red_in_clos_trans_par_red.
 Qed.
-
-(* TODO:
-  (1) P ⇛ P' -> (forall x, σ_1 x !⇛ σ_2 x) -> P[σ_1] ⊵ P'[σ_2]
-  (2) P ⊵ P' -> (forall x, σ_1 x !⇛ σ_2 x) -> P[σ_1] ⊵ P'[σ_2]
-  (not sure if induction suffices or induction on depth)
-*)
