formalization/Confluence.v
@@ -8,39 +8,24 @@ From FD Require Import DirectedCong.
 From FD Require Import Reduction.
 From FD Require Import ParallelReduction.
 
-Lemma diamond_par_red_imp_diamond_multistep :
-  diamond_property par_reduces -> diamond_property multi_step_reduction.
-Proof.
-  intros. apply diamond_R_diamond_clos_trans_R in H.
-  eapply diamond_preserved_under_eq; eauto.
-  apply par_reds_clos_trans_multi_step_red_coincide.
-Qed.
-
-Lemma link_directed_cong_par_red_confluent :
+Lemma link_directed_cong_equiv_red_commute :
   forall ml mr P Q, (link ml mr) ⇛ P -> (link ml mr) ⊵ Q ->
-    exists R, P ⊵ R /\ Q ⊵ R.
+    exists R, P ⊵ R /\ Q ⇛ R.
 Proof.
-  intros. inversion H; subst.
-  { exists Q; split; auto; econstructor. econstructor. }
-  inversion H0; subst;
-  (* For reflexivity, we discharge the goal via admissibility of symmetry *)
-  try (now (eexists; split; econstructor; apply directed_cong_symm; eauto));
+  intros. inversion H; inversion H0; subst;
   try match goal with
-  | [ H1 : (prefix (send _ _)) !⇛ _,
+  | [ H1 : (prefix (send _ _))  !⇛ _,
       H2 : (prefix (receive _)) !⇛ _
       |- _ ] =>
     apply directed_cong_inversion_prefix in H1; destruct H1 as [? [? H1']];
     apply directed_cong_inversion_prefix in H2; destruct H2 as [? [? H2']];
     apply directed_cong_inversion_send in H1'; destruct H1' as [? [? [? [? ?]]]];
     apply directed_cong_inversion_receive in H2'; destruct H2' as [? [? ?]];
-    subst; eexists; split; [
-      try eapply rp_tensor_par_2; try eapply rp_tensor_par_1; try eapply directed_cong_symm; eauto
-    | eapply rp_cong_cut; try (now (econstructor; eapply directed_cong_symm; eauto));
-      eapply rp_cong_cut; try (now (econstructor; eapply directed_cong_symm; eauto));
-      econstructor; apply directed_cong_invariant_under_renaming; try apply swap01_is_bijective;
-      apply directed_cong_invariant_under_upshifting;
-      apply directed_cong_symm; auto
-    ]
+    subst; eexists; split; 
+    [ try eapply rp_tensor_par_1; try eapply rp_tensor_par_2; auto
+    | apply dc_cong_cut; auto; apply dc_cong_cut; auto;
+      apply directed_cong_invariant_under_renaming; try apply swap01_is_bijective;
+      apply directed_cong_invariant_under_upshifting; auto ]
   | [ H1 : (prefix (choose_left _)) !⇛ _,
       H2 : (prefix (offer_choice _ _)) !⇛ _
       |- _ ] =>
@@ -48,14 +33,11 @@ Proof.
     apply directed_cong_inversion_prefix in H2; destruct H2 as [? [? H2']];
     apply directed_cong_inversion_choosel in H1'; destruct H1' as [? [? ?]];
     apply directed_cong_inversion_choice in H2'; destruct H2' as [? [? [? [? ?]]]];
-    subst; eexists; split; [
-      try eapply rp_plus_with_l1; try eapply rp_plus_with_l2; try eapply directed_cong_symm; eauto
-    | eapply rp_cong_cut; try (now (econstructor; eapply directed_cong_symm; eauto));
-      eapply rp_cong_cut; try (now (econstructor; eapply directed_cong_symm; eauto));
-      econstructor; apply directed_cong_invariant_under_renaming; try apply swap01_is_bijective;
-      apply directed_cong_invariant_under_upshifting;
-      apply directed_cong_symm; auto
-    ]
+    subst; eexists; split; 
+    [ try eapply rp_plus_with_l1; try eapply rp_plus_with_l2; auto
+    | apply dc_cong_cut; auto; apply dc_cong_cut; auto;
+      apply directed_cong_invariant_under_renaming; try apply swap01_is_bijective;
+      apply directed_cong_invariant_under_upshifting; auto ]
   | [ H1 : (prefix (choose_right _)) !⇛ _,
       H2 : (prefix (offer_choice _ _)) !⇛ _
       |- _ ] =>
@@ -63,14 +45,11 @@ Proof.
     apply directed_cong_inversion_prefix in H2; destruct H2 as [? [? H2']];
     apply directed_cong_inversion_chooser in H1'; destruct H1' as [? [? ?]];
     apply directed_cong_inversion_choice in H2'; destruct H2' as [? [? [? [? ?]]]];
-    subst; eexists; split; [
-      try eapply rp_plus_with_r1; try eapply rp_plus_with_r2; try eapply directed_cong_symm; eauto
-    | eapply rp_cong_cut; try (now (econstructor; eapply directed_cong_symm; eauto));
-      eapply rp_cong_cut; try (now (econstructor; eapply directed_cong_symm; eauto));
-      econstructor; apply directed_cong_invariant_under_renaming; try apply swap01_is_bijective;
-      apply directed_cong_invariant_under_upshifting;
-      apply directed_cong_symm; auto
-    ]
+    subst; eexists; split; 
+    [ try eapply rp_plus_with_r1; try eapply rp_plus_with_r2; auto
+    | apply dc_cong_cut; auto; apply dc_cong_cut; auto;
+      apply directed_cong_invariant_under_renaming; try apply swap01_is_bijective;
+      apply directed_cong_invariant_under_upshifting; auto ]
   | [ H1 : (prefix close) !⇛ _,
       H2 : (prefix (wait _)) !⇛ _
       |- _ ] =>
@@ -78,76 +57,134 @@ Proof.
     apply directed_cong_inversion_prefix in H2; destruct H2 as [? [? H2']];
     apply directed_cong_inversion_close in H1';
     apply directed_cong_inversion_wait in H2'; destruct H2' as [? [? ?]];
-    subst; eexists; split; [
-      try eapply rp_one_bot1; try eapply rp_one_bot2; try eapply directed_cong_symm; eauto
-    | econstructor; apply directed_cong_symm; auto
-    ]
+    subst; eexists; split; [ try eapply rp_one_bot1; try eapply rp_one_bot2; eauto | auto ]
   end.
+  + eexists. split. apply rp_refl. apply dc_cong_link; auto.
+  + inversion H; subst.
+    - eexists. split. apply rp_refl. econstructor; auto.
+    - eexists. split. apply rp_refl. apply dc_link; auto.
 Qed.
 
-Lemma confluence_directed_cong_par_red :
-  forall P Q1 Q2, P ⇛ Q1 -> P ⊵ Q2 -> exists R, Q1 ⊵ R /\ Q2 ⊵ R.
+(* ⇛ and ⊵ commute *)
+(*
+         P
+      ⇛    ⊵
+    Q1       Q2
+      ⊵    ⇛
+         R
+*)
+Lemma directed_cong_equiv_red_commute :
+  (* ⇛ in conclusion has to be changed to ≡ for axcut *)
+  forall P Q1 Q2, P ⇛ Q1 -> P ⊵ Q2 -> exists R, Q1 ⊵ R /\ Q2 ⇛ R.
 Proof.
   intros. generalize dependent Q2.
   induction H; intros.
-  + exists Q2. split; auto. econstructor. apply c_refl.
-  + eapply link_directed_cong_par_red_confluent; eauto. econstructor; eauto.
-  + inversion H1; subst.
-    - admit.
-    - (* downM M' requires well-typedness of M to conclude that 0 is not in free vars of M' *)
-      admit.
-    - admit.
-    - inversion H0; subst.
-      * (* cut (cut (link (future 1) M) R) P2
-           not covered by parallel reduction
-           NB: try approach below before adding addtional reduction rules and
-               see how far we can go. However, we will likely need all
-               rp_cut_assoc rules up to symmetry (see original approach)
-               with this addtional premise
-        *)
-        (* add a premise:
-            L ⇛ (cut (link (future 1) M) R)
-           to rp_ax_cut_assoc rules so that
-           cut P L ⊵ cut (subst_process P'' ((downM M'' ⋅ id_subst))) R''
-        *)
+  (* link *)
+  + eapply link_directed_cong_equiv_red_commute; eauto; econstructor; eauto.
+  + eapply link_directed_cong_equiv_red_commute; eauto. apply dc_link; auto.
+
+  (* cut *)
+  + admit.
+  + admit.
+  + admit.
+  + admit.
+
+  (* + inversion H0; subst.
+    - eexists. split. econstructor. apply dc_cut_comm.
+    - eexists. split.
+      * apply rp_cong_cut_r; eauto.
+      * apply dc_cut_comm.
+    - eexists. split.
+      * apply rp_cong_cut_l; eauto.
+      * apply dc_cut_comm.
+  + inversion H3; subst.
+    - eexists. split.
+      * apply rp_refl.
+      * eapply dc_cut_assoc_l; auto.
+    - inversion H7; subst.
+      *  eexists. split. apply rp_refl. apply dc_cut_assoc_l; auto.
+      * (* ⊵ is invariant under renaming, shifting *)
+        assert ( (down (rename_process P swap01)) ⊵  (down (rename_process P' swap01)) )
+         by admit.
+        eexists. split. { apply rp_cong_cut_l. apply H0. }
+        apply dc_cut_assoc_l; auto.
+        (* free variables are preserved under reduction *)
         admit.
-      * admit.
-      * (* congruences allows to perform association more than once !!!!! *)
-        admit.
-    - inversion H; subst.
-      * admit.
-      * admit. (* should work easily with new premise *)
-      * admit.
-    - admit.
-  + inversion H6; subst.
-    - exists Q2; split; try (now econstructor);
-      admit.
-    - (* dont bother doing an inversion on H9; try to use invariances instead *)
-      (* we need 0 not in M/M' *)
-      admit.
-    - (* in R1, up results in future 2 but swap01 is also uped ->
-         future 1 remains in R1 ->
-         via cut_cong, the left side may still reduce via cut assoc
-         use H9 and invariances too conclude result
-         *)
-      admit.
-    - admit.
+      * (* ⊵ is invariant under renaming, shifting *)
+        assert ( (rename_process Q swap01) ⊵  (rename_process Q' swap01) )
+         by admit.
+        eexists. split. { apply rp_cong_cut_r. apply rp_cong_cut_l. apply H0. }
+        apply dc_cut_assoc_l; auto.
     - admit.
   + admit.
+  + admit. *)
+
+  (* seq *)
   + inversion H1; subst.
-    - exists (seq P s). apply directed_cong_symm in H, H0, H2.
-      split; auto; repeat econstructor; auto.
-    - eexists. split.
-      * eapply rp_seq.
-        { apply directed_cong_symm in H. apply H. }
-        { apply directed_cong_symm in H0. apply H0. }
-      * apply directed_cong_symm in H4, H6. econstructor.
-        apply directed_cong_substitution; auto.
-        intros i. destruct i; simpl; econstructor; auto.
-    - apply directed_cong_symm in H, H0, H6.
-      apply IHdirected_congruence in H4. destruct H4 as [? [? ?]].
-      eexists. split; eapply rp_cong_seq; eauto.
+    - eexists. split. apply rp_refl. apply dc_cong_seq; auto.
+    - eexists. split. apply rp_seq.
+      apply directed_cong_invariant_under_substitution; auto.
+      intros [|]; simpl. { econstructor; eauto. }
+      apply dc_cong_reflM.
+    - destruct (IHdirected_congruence _ H5) as [? [? ?]].
+      eexists. split.
+      * apply rp_cong_seq. apply H2.
+      * apply dc_cong_seq; auto.
+  + inversion H0; subst. exists stop; split; eauto. apply dc_stop.
 Admitted.
+
+(* ≡ and ↠ commute *)
+(*
+         P
+      ≡    ↠
+    Q1       Q2
+      ↠    ≡
+         R
+*)
+Lemma struct_cong_par_red_commute :
+  forall P Q1 Q2, P ≡ Q1 -> P ↠ Q2 -> exists R, Q1 ↠ R /\ Q2 ≡ R.
+Proof.
+  intros. destruct H0.
+  + apply struct_cong_in_trans_directed_cong in H.
+    generalize dependent Q2.
+    induction H; intros.
+    - destruct (directed_cong_equiv_red_commute _ _ _ H H0) as [? [? ?]].
+      exists x0. split.
+      * left. auto.
+      * apply directed_cong_in_struct_cong. auto.
+    - destruct (directed_cong_equiv_red_commute _ _ _ H H1) as [? [? ?]].
+      destruct (IHclos_trans_1n _ H2) as [? [? ?]].
+      exists x1. split; auto.
+      apply directed_cong_in_struct_cong in H3. eapply c_trans; eauto.
+  + exists P. split.
+    - right. apply c_comm; auto.
+    - apply c_comm; auto.
+Qed.
+
+(* ↠ is confluent *)
+Lemma church_rosser_parallel_reduction :
+  diamond_property par_reduction.
+Proof.
+  unfold diamond_property. intros.
+  destruct H eqn:E.
+  + destruct H0.
+    - clear - H0 e.
+      admit.
+    - destruct (struct_cong_par_red_commute _ _ _ H0 H) as [? [? ?]].
+      eexists; split; eauto. right; auto.
+  + destruct (struct_cong_par_red_commute _ _ _ s H0) as [? [? ?]].
+    eexists; split; eauto. right; auto.
+Admitted.
+
+(* ▶ is confluent *)
+Lemma church_rosser :
+  diamond_property multi_step_reduction.
+Proof.
+  eapply diamond_preserved_under_eq.
+  + apply diamond_R_diamond_clos_trans_R.
+    apply church_rosser_parallel_reduction.
+  + apply par_reds_clos_trans_multi_step_red_coincide.
+Qed.
 
 (* invariance for ⊵ under renaming, shifting, substitution must follow by induction on depth *)
 (* for invariance under subst: show that subst compose then argue by extensionality on composition 
